<?xml version="1.0"?>
<rdf:RDF xmlns="https://w3id.org/ecodigit/ontology/eas/"
     xml:base="https://w3id.org/ecodigit/ontology/eas/"
     xmlns:dc="http://purl.org/dc/elements/1.1/"
     xmlns:l0="https://w3id.org/italia/onto/l0/"
     xmlns:ns="http://www.w3.org/2003/06/sw-vocab-status/ns#"
     xmlns:CLV="https://w3id.org/italia/onto/CLV/"
     xmlns:ns1="http://www.w3.org/2006/vcard/ns#"
     xmlns:org="http://www.w3.org/ns/org#"
     xmlns:owl="http://www.w3.org/2002/07/owl#"
     xmlns:rdf="http://www.w3.org/1999/02/22-rdf-syntax-ns#"
     xmlns:wot="http://xmlns.com/wot/0.1/"
     xmlns:xml="http://www.w3.org/XML/1998/namespace"
     xmlns:xsd="http://www.w3.org/2001/XMLSchema#"
     xmlns:ADMS="https://w3id.org/italia/onto/ADMS/"
     xmlns:dcat="http://www.w3.org/ns/dcat#"
     xmlns:foaf="http://xmlns.com/foaf/0.1/"
     xmlns:prov="http://www.w3.org/ns/prov#"
     xmlns:rdfs="http://www.w3.org/2000/01/rdf-schema#"
     xmlns:skos="http://www.w3.org/2004/02/skos/core#"
     xmlns:terms="http://purl.org/dc/terms/"
     xmlns:owlapi="http://www.semanticweb.org/owlapi#"
     xmlns:ecodigit-eas="https://w3id.org/ecodigit/ontology/eas/"
     xmlns:cpannotationschema="http://www.ontologydesignpatterns.org/schemas/cpannotationschema.owl#">
    <owl:Ontology rdf:about="https://w3id.org/ecodigit/ontology/eas/">
        <owl:versionIRI rdf:resource="https://w3id.org/ecodigit/ontology/eas/0.2/"/>
        <owl:imports rdf:resource="http://purl.org/ontology/bibo/"/>
        <owl:imports rdf:resource="https://w3id.org/ecodigit/ontology/grade"/>
        <owl:imports rdf:resource="https://w3id.org/ecodigit/ontology/organization"/>
        <owl:imports rdf:resource="https://w3id.org/italia/onto/CPV-aligns"/>
        <owl:imports rdf:resource="https://w3id.org/italia/onto/Language"/>
        <dc:description rdf:resource="https://raw.githubusercontent.com/ecodigit/workspace/master/ontology/eas/0.01/diagram.png"/>
    </owl:Ontology>
    


    <!-- 
    ///////////////////////////////////////////////////////////////////////////////////////
    //
    // Object Properties
    //
    ///////////////////////////////////////////////////////////////////////////////////////
     -->

    


    <!-- https://w3id.org/ecodigit/ontology/eas/attends -->

    <owl:ObjectProperty rdf:about="https://w3id.org/ecodigit/ontology/eas/attends">
        <owl:inverseOf rdf:resource="https://w3id.org/ecodigit/ontology/eas/isAttendedBy"/>
        <rdfs:domain rdf:resource="https://w3id.org/italia/onto/CPV/Person"/>
        <rdfs:range rdf:resource="https://w3id.org/ecodigit/ontology/eas/Training"/>
        <rdfs:comment xml:lang="it">Questa proprietà permette di associare una Persona con l&apos;Esperienza formativa da essa frequentata.</rdfs:comment>
        <rdfs:comment xml:lang="en">This property associates a Person with the attended Training.</rdfs:comment>
        <rdfs:isDefinedBy rdf:resource="https://w3id.org/ecodigit/ontology/eas/"/>
        <rdfs:label xml:lang="en">attends</rdfs:label>
        <rdfs:label xml:lang="it">frequenta</rdfs:label>
        <owl:versionInfo xml:lang="it">stabile</owl:versionInfo>
        <owl:versionInfo xml:lang="en">stable</owl:versionInfo>
    </owl:ObjectProperty>
    


    <!-- https://w3id.org/ecodigit/ontology/eas/attests -->

    <owl:ObjectProperty rdf:about="https://w3id.org/ecodigit/ontology/eas/attests">
        <owl:inverseOf rdf:resource="https://w3id.org/ecodigit/ontology/eas/isAttestedBy"/>
        <rdfs:domain rdf:resource="https://w3id.org/ecodigit/ontology/eas/Certification"/>
        <rdfs:range rdf:resource="https://w3id.org/italia/onto/l0/Characteristic"/>
        <rdfs:comment xml:lang="it">Questa proprietà permette di associare una Certificazione con il Livello di competenza attestato.</rdfs:comment>
        <rdfs:comment xml:lang="en">This property associates a Certification with the attested Level of Expertise.</rdfs:comment>
        <rdfs:isDefinedBy rdf:resource="https://w3id.org/ecodigit/ontology/eas/"/>
        <rdfs:label xml:lang="it">attesta</rdfs:label>
        <rdfs:label xml:lang="en">attests</rdfs:label>
        <owl:versionInfo xml:lang="it">stabile</owl:versionInfo>
        <owl:versionInfo xml:lang="en">stable</owl:versionInfo>
    </owl:ObjectProperty>
    


    <!-- https://w3id.org/ecodigit/ontology/eas/hasActivity -->

    <owl:ObjectProperty rdf:about="https://w3id.org/ecodigit/ontology/eas/hasActivity">
        <rdfs:domain rdf:resource="https://w3id.org/ecodigit/ontology/eas/LevelInActivity"/>
        <rdfs:range rdf:resource="https://w3id.org/italia/onto/l0/Activity"/>
        <rdfs:comment xml:lang="it">Questa proprietà associa il Livello in Attività con l&apos;attività a cui si riferisce.</rdfs:comment>
        <rdfs:comment xml:lang="en">This property associates the Level in Activity with the activity it refers to.</rdfs:comment>
        <rdfs:isDefinedBy rdf:resource="https://w3id.org/ecodigit/ontology/eas/"/>
        <rdfs:label xml:lang="it">ha attività</rdfs:label>
        <rdfs:label xml:lang="en">has activity</rdfs:label>
        <owl:versionInfo xml:lang="it">stabile</owl:versionInfo>
        <owl:versionInfo xml:lang="en">stable</owl:versionInfo>
    </owl:ObjectProperty>
    


    <!-- https://w3id.org/ecodigit/ontology/eas/hasCertification -->

    <owl:ObjectProperty rdf:about="https://w3id.org/ecodigit/ontology/eas/hasCertification">
        <owl:inverseOf rdf:resource="https://w3id.org/ecodigit/ontology/eas/isCertificationOf"/>
        <rdfs:domain rdf:resource="http://www.w3.org/2002/07/owl#Thing"/>
        <rdfs:range rdf:resource="https://w3id.org/ecodigit/ontology/eas/Certification"/>
        <rdfs:comment xml:lang="it">Questa proprietà associa una Entità alla sua Certificazione sia essa istituzionale o autodichiarata.</rdfs:comment>
        <rdfs:comment xml:lang="en">This property associates an Entity with its Certification whether it is institutional or self-declared.</rdfs:comment>
        <rdfs:isDefinedBy rdf:resource="https://w3id.org/ecodigit/ontology/eas/"/>
        <rdfs:label xml:lang="it">ha certificazione</rdfs:label>
        <rdfs:label xml:lang="en">has certification</rdfs:label>
        <owl:versionInfo xml:lang="it">stabile</owl:versionInfo>
        <owl:versionInfo xml:lang="en">stable</owl:versionInfo>
    </owl:ObjectProperty>
    


    <!-- https://w3id.org/ecodigit/ontology/eas/hasCertifiedExpertiseLevel -->

    <owl:ObjectProperty rdf:about="https://w3id.org/ecodigit/ontology/eas/hasCertifiedExpertiseLevel">
        <rdfs:domain rdf:resource="https://w3id.org/ecodigit/ontology/eas/LevelInActivity"/>
        <rdfs:range rdf:resource="https://w3id.org/ecodigit/ontology/eas/CertifiedExpertiseLevel"/>
        <rdfs:comment xml:lang="it">Questa proprietà associa un Livello in Attività con il Livello certificato dell&apos;esperienza a cui si riferisce.</rdfs:comment>
        <rdfs:comment xml:lang="en">This property associates an Activity Level with the Certified Expertise Level it refers to.</rdfs:comment>
        <rdfs:isDefinedBy rdf:resource="https://w3id.org/ecodigit/ontology/eas/"/>
        <rdfs:label xml:lang="it">ha livello</rdfs:label>
        <rdfs:label xml:lang="en">has level</rdfs:label>
        <owl:versionInfo xml:lang="it">stabile</owl:versionInfo>
        <owl:versionInfo xml:lang="en">stable</owl:versionInfo>
    </owl:ObjectProperty>
    


    <!-- https://w3id.org/ecodigit/ontology/eas/hasExpertise -->

    <owl:ObjectProperty rdf:about="https://w3id.org/ecodigit/ontology/eas/hasExpertise">
        <rdfs:domain rdf:resource="https://w3id.org/italia/onto/CPV/Person"/>
        <rdfs:range rdf:resource="https://w3id.org/ecodigit/ontology/eas/Expertise"/>
        <rdfs:comment xml:lang="it">Questa proprietà associa una Persona con la sua Esperienza o Competenza.</rdfs:comment>
        <rdfs:comment xml:lang="en">This property associates a Person with his Expertise or Competence.</rdfs:comment>
        <rdfs:isDefinedBy rdf:resource="https://w3id.org/ecodigit/ontology/eas/"/>
        <rdfs:label xml:lang="it">ha esperienza</rdfs:label>
        <rdfs:label xml:lang="en">has expertise</rdfs:label>
        <owl:versionInfo xml:lang="it">stabile</owl:versionInfo>
        <owl:versionInfo xml:lang="en">stable</owl:versionInfo>
        <prov:wasInfluencedBy rdf:resource="http://purl.org/ontology/cco/core#expertise"/>
    </owl:ObjectProperty>
    


    <!-- https://w3id.org/ecodigit/ontology/eas/hasTrainingOutcome -->

    <owl:ObjectProperty rdf:about="https://w3id.org/ecodigit/ontology/eas/hasTrainingOutcome">
        <owl:inverseOf rdf:resource="https://w3id.org/ecodigit/ontology/eas/isTrainingOutcomeOf"/>
        <rdfs:domain>
            <owl:Class>
                <owl:unionOf rdf:parseType="Collection">
                    <rdf:Description rdf:about="https://w3id.org/ecodigit/ontology/eas/Examination"/>
                    <rdf:Description rdf:about="https://w3id.org/ecodigit/ontology/eas/Training"/>
                </owl:unionOf>
            </owl:Class>
        </rdfs:domain>
        <rdfs:range rdf:resource="http://www.w3.org/2002/07/owl#Thing"/>
        <rdfs:comment xml:lang="it">Questa proprietà associa un&apos;Esperienza formativa o un Esame con qualsiasi cosa sia il risultato della formazione (ad es. una Tesi).</rdfs:comment>
        <rdfs:comment xml:lang="en">This property associates a Training experience or an Examination  with anything is the result of the training (e.g. a Thesis).</rdfs:comment>
        <rdfs:isDefinedBy rdf:resource="https://w3id.org/ecodigit/ontology/eas/"/>
        <rdfs:label xml:lang="it">ha risultato della formazione</rdfs:label>
        <rdfs:label xml:lang="en">has training outcome</rdfs:label>
        <owl:versionInfo xml:lang="it">stabile</owl:versionInfo>
        <owl:versionInfo xml:lang="en">stable</owl:versionInfo>
    </owl:ObjectProperty>
    


    <!-- https://w3id.org/ecodigit/ontology/eas/includesAnExamination -->

    <owl:ObjectProperty rdf:about="https://w3id.org/ecodigit/ontology/eas/includesAnExamination">
        <rdfs:domain rdf:resource="https://w3id.org/ecodigit/ontology/eas/Training"/>
        <rdfs:range rdf:resource="https://w3id.org/ecodigit/ontology/eas/Examination"/>
        <rdfs:comment xml:lang="it">La proprietà permette di associare una Esperienza formativa con gli esami necessari per il suo completamento.</rdfs:comment>
        <rdfs:comment xml:lang="en">The property associates a Training with the Examinations required for its completion.</rdfs:comment>
        <rdfs:isDefinedBy rdf:resource="https://w3id.org/ecodigit/ontology/eas/"/>
        <rdfs:label xml:lang="it">include un esame</rdfs:label>
        <rdfs:label xml:lang="en">includes an examination</rdfs:label>
        <owl:versionInfo xml:lang="it">stabile</owl:versionInfo>
        <owl:versionInfo xml:lang="en">stable</owl:versionInfo>
    </owl:ObjectProperty>
    


    <!-- https://w3id.org/ecodigit/ontology/eas/isAttendedBy -->

    <owl:ObjectProperty rdf:about="https://w3id.org/ecodigit/ontology/eas/isAttendedBy">
        <rdfs:domain rdf:resource="https://w3id.org/ecodigit/ontology/eas/Training"/>
        <rdfs:range rdf:resource="https://w3id.org/italia/onto/CPV/Person"/>
        <rdfs:comment xml:lang="it">Questa è la proprietà inversa di &apos;frequenta&apos;.</rdfs:comment>
        <rdfs:comment xml:lang="en">This is the inverse object property of &apos;attends&apos;.</rdfs:comment>
        <rdfs:isDefinedBy rdf:resource="https://w3id.org/ecodigit/ontology/eas/"/>
        <rdfs:label xml:lang="en">is attended by</rdfs:label>
        <rdfs:label xml:lang="it">è frequentato da</rdfs:label>
        <owl:versionInfo xml:lang="it">stabile</owl:versionInfo>
        <owl:versionInfo xml:lang="en">stable</owl:versionInfo>
    </owl:ObjectProperty>
    


    <!-- https://w3id.org/ecodigit/ontology/eas/isAttestedBy -->

    <owl:ObjectProperty rdf:about="https://w3id.org/ecodigit/ontology/eas/isAttestedBy">
        <rdfs:domain rdf:resource="https://w3id.org/italia/onto/l0/Characteristic"/>
        <rdfs:range rdf:resource="https://w3id.org/ecodigit/ontology/eas/Certification"/>
        <rdfs:comment xml:lang="it">Questa è la proprietà inversa di &apos;attesta&apos;.</rdfs:comment>
        <rdfs:comment xml:lang="en">This is the inverse object property of &apos;attests&apos;.</rdfs:comment>
        <rdfs:isDefinedBy rdf:resource="https://w3id.org/ecodigit/ontology/eas/"/>
        <rdfs:label xml:lang="en">is attested by</rdfs:label>
        <rdfs:label xml:lang="it">è attestato da</rdfs:label>
        <owl:versionInfo xml:lang="it">stabile</owl:versionInfo>
        <owl:versionInfo xml:lang="en">stable</owl:versionInfo>
    </owl:ObjectProperty>
    


    <!-- https://w3id.org/ecodigit/ontology/eas/isCertificationOf -->

    <owl:ObjectProperty rdf:about="https://w3id.org/ecodigit/ontology/eas/isCertificationOf">
        <rdfs:domain rdf:resource="https://w3id.org/ecodigit/ontology/eas/Certification"/>
        <rdfs:range rdf:resource="http://www.w3.org/2002/07/owl#Thing"/>
        <rdfs:comment xml:lang="it">Questa è la proprietà inversa di &apos;ha certificazione&apos;.</rdfs:comment>
        <rdfs:comment xml:lang="en">This is the inverse object property of &apos;has certification&apos;.</rdfs:comment>
        <rdfs:isDefinedBy rdf:resource="https://w3id.org/ecodigit/ontology/eas/"/>
        <rdfs:label xml:lang="en">is certification of</rdfs:label>
        <rdfs:label xml:lang="it">è certificazione di</rdfs:label>
        <owl:versionInfo xml:lang="it">stabile</owl:versionInfo>
        <owl:versionInfo xml:lang="en">stable</owl:versionInfo>
    </owl:ObjectProperty>
    


    <!-- https://w3id.org/ecodigit/ontology/eas/isTrainingOutcomeOf -->

    <owl:ObjectProperty rdf:about="https://w3id.org/ecodigit/ontology/eas/isTrainingOutcomeOf">
        <rdfs:domain rdf:resource="http://www.w3.org/2002/07/owl#Thing"/>
        <rdfs:range>
            <owl:Class>
                <owl:unionOf rdf:parseType="Collection">
                    <rdf:Description rdf:about="https://w3id.org/ecodigit/ontology/eas/Examination"/>
                    <rdf:Description rdf:about="https://w3id.org/ecodigit/ontology/eas/Training"/>
                </owl:unionOf>
            </owl:Class>
        </rdfs:range>
        <rdfs:comment xml:lang="it">Questa è la proprietà inversa di &apos;ha risultato della formazione&apos;.</rdfs:comment>
        <rdfs:comment xml:lang="en">This is the inverse object property of &apos;has training outcome&apos;.</rdfs:comment>
        <rdfs:isDefinedBy rdf:resource="https://w3id.org/ecodigit/ontology/eas/"/>
        <rdfs:label xml:lang="en">is training outcome of</rdfs:label>
        <rdfs:label xml:lang="it">è risultato della formazione di</rdfs:label>
        <owl:versionInfo xml:lang="it">stabile</owl:versionInfo>
        <owl:versionInfo xml:lang="en">stable</owl:versionInfo>
    </owl:ObjectProperty>
    


    <!-- https://w3id.org/ecodigit/ontology/eas/issuedBy -->

    <owl:ObjectProperty rdf:about="https://w3id.org/ecodigit/ontology/eas/issuedBy">
        <owl:inverseOf rdf:resource="https://w3id.org/ecodigit/ontology/eas/issues"/>
        <rdfs:domain rdf:resource="https://w3id.org/ecodigit/ontology/eas/Certification"/>
        <rdfs:range rdf:resource="https://w3id.org/italia/onto/COV/Organization"/>
        <rdfs:comment xml:lang="it">Questa proprietà associa una Certificazione con l&apos;Organizzazione che la rilascia.</rdfs:comment>
        <rdfs:comment xml:lang="en">This property associates a Certification with the issuing Organization.</rdfs:comment>
        <rdfs:isDefinedBy rdf:resource="https://w3id.org/ecodigit/ontology/eas/"/>
        <rdfs:label xml:lang="en">certification issued by</rdfs:label>
        <rdfs:label xml:lang="it">certificazione rilasciata da</rdfs:label>
        <owl:versionInfo xml:lang="it">stabile</owl:versionInfo>
        <owl:versionInfo xml:lang="en">stable</owl:versionInfo>
    </owl:ObjectProperty>
    


    <!-- https://w3id.org/ecodigit/ontology/eas/issues -->

    <owl:ObjectProperty rdf:about="https://w3id.org/ecodigit/ontology/eas/issues">
        <rdfs:domain rdf:resource="https://w3id.org/italia/onto/COV/Organization"/>
        <rdfs:range rdf:resource="https://w3id.org/ecodigit/ontology/eas/Certification"/>
        <rdfs:comment xml:lang="it">Questa proprietà associa un&apos;Organizzazione con la Certificazione che essa rilascia.</rdfs:comment>
        <rdfs:comment xml:lang="en">This property associates an Organization with the Certification that it issues.</rdfs:comment>
        <rdfs:isDefinedBy rdf:resource="https://w3id.org/ecodigit/ontology/eas/"/>
        <rdfs:label xml:lang="en">issues certification</rdfs:label>
        <rdfs:label xml:lang="it">rilascia certificazione</rdfs:label>
        <owl:versionInfo xml:lang="it">stabile</owl:versionInfo>
        <owl:versionInfo xml:lang="en">stable</owl:versionInfo>
    </owl:ObjectProperty>
    


    <!-- https://w3id.org/ecodigit/ontology/eas/leadsTo -->

    <owl:ObjectProperty rdf:about="https://w3id.org/ecodigit/ontology/eas/leadsTo">
        <rdfs:domain rdf:resource="https://w3id.org/ecodigit/ontology/eas/Examination"/>
        <rdfs:range rdf:resource="https://w3id.org/ecodigit/ontology/eas/Certification"/>
        <rdfs:comment xml:lang="it">Questa proprietà permette di associare la situazione del superamento di un Esame con la Certificazione ottenuta.</rdfs:comment>
        <rdfs:comment xml:lang="en">This property allows you to associate the situation of passing an Exam with the Certification obtained.</rdfs:comment>
        <rdfs:isDefinedBy rdf:resource="https://w3id.org/ecodigit/ontology/eas/"/>
        <rdfs:label xml:lang="en">leads to the achievement of</rdfs:label>
        <rdfs:label xml:lang="it">porta al conseguimento di</rdfs:label>
        <owl:versionInfo xml:lang="it">stabile</owl:versionInfo>
        <owl:versionInfo xml:lang="en">stable</owl:versionInfo>
    </owl:ObjectProperty>
    


    <!-- https://w3id.org/ecodigit/ontology/eas/providedBy -->

    <owl:ObjectProperty rdf:about="https://w3id.org/ecodigit/ontology/eas/providedBy">
        <owl:inverseOf rdf:resource="https://w3id.org/ecodigit/ontology/eas/provides"/>
        <rdfs:domain rdf:resource="https://w3id.org/ecodigit/ontology/eas/Training"/>
        <rdfs:range rdf:resource="https://w3id.org/italia/onto/COV/Organization"/>
        <rdfs:comment xml:lang="it">Questa proprietà permette di associare una situazione di Formazione con l&apos;Organizzazione che la eroga.</rdfs:comment>
        <rdfs:comment xml:lang="en">This property associates a Training situation with the Organization providing it.</rdfs:comment>
        <rdfs:isDefinedBy rdf:resource="https://w3id.org/ecodigit/ontology/eas/"/>
        <rdfs:label xml:lang="it">offerta da</rdfs:label>
        <rdfs:label xml:lang="en">provided by</rdfs:label>
        <owl:versionInfo xml:lang="it">stabile</owl:versionInfo>
        <owl:versionInfo xml:lang="en">stable</owl:versionInfo>
    </owl:ObjectProperty>
    


    <!-- https://w3id.org/ecodigit/ontology/eas/provides -->

    <owl:ObjectProperty rdf:about="https://w3id.org/ecodigit/ontology/eas/provides">
        <rdfs:domain rdf:resource="https://w3id.org/italia/onto/COV/Organization"/>
        <rdfs:range rdf:resource="https://w3id.org/ecodigit/ontology/eas/Training"/>
        <rdfs:comment xml:lang="it">Questa è la proprietà inversa di &apos;è offerta da&apos;.</rdfs:comment>
        <rdfs:comment xml:lang="en">This is the inverse object property of &apos;provided by&apos;.</rdfs:comment>
        <rdfs:isDefinedBy rdf:resource="https://w3id.org/ecodigit/ontology/eas/"/>
        <rdfs:label xml:lang="it">offre</rdfs:label>
        <rdfs:label xml:lang="en">provides</rdfs:label>
        <owl:versionInfo xml:lang="it">stabile</owl:versionInfo>
        <owl:versionInfo xml:lang="en">stable</owl:versionInfo>
    </owl:ObjectProperty>
    


    <!-- 
    ///////////////////////////////////////////////////////////////////////////////////////
    //
    // Data properties
    //
    ///////////////////////////////////////////////////////////////////////////////////////
     -->

    


    <!-- https://w3id.org/ecodigit/ontology/eas/issueDate -->

    <owl:DatatypeProperty rdf:about="https://w3id.org/ecodigit/ontology/eas/issueDate">
        <rdfs:subPropertyOf rdf:resource="https://w3id.org/italia/onto/TI/date"/>
        <rdfs:domain rdf:resource="https://w3id.org/ecodigit/ontology/eas/Certification"/>
        <rdfs:range rdf:resource="http://www.w3.org/2001/XMLSchema#date"/>
        <rdfs:comment xml:lang="it">Questa proprietà rappresenta la data di rilascio della Certificazione.</rdfs:comment>
        <rdfs:comment xml:lang="en">This property represents the issue date of the Certification.</rdfs:comment>
        <rdfs:isDefinedBy rdf:resource="https://w3id.org/ecodigit/ontology/eas/"/>
        <rdfs:label xml:lang="it">data di rilascio</rdfs:label>
        <rdfs:label xml:lang="en">issue date</rdfs:label>
        <owl:versionInfo xml:lang="it">stabile</owl:versionInfo>
        <owl:versionInfo xml:lang="en">stable</owl:versionInfo>
    </owl:DatatypeProperty>
    


    <!-- 
    ///////////////////////////////////////////////////////////////////////////////////////
    //
    // Classes
    //
    ///////////////////////////////////////////////////////////////////////////////////////
     -->

    


    <!-- http://purl.org/ontology/bibo/Thesis -->

    <owl:Class rdf:about="http://purl.org/ontology/bibo/Thesis"/>
    


    <!-- http://xmlns.com/foaf/0.1/Agent -->

    <owl:Class rdf:about="http://xmlns.com/foaf/0.1/Agent"/>
    


    <!-- https://w3id.org/ecodigit/ontology/eas/CERFLevel -->

    <owl:Class rdf:about="https://w3id.org/ecodigit/ontology/eas/CERFLevel">
        <rdfs:subClassOf rdf:resource="https://w3id.org/ecodigit/ontology/eas/CertifiedExpertiseLevel"/>
        <rdfs:comment xml:lang="it">Questa classe rappresenta i sei livelli (A1, A2, B1, B2, C1, C2) previsti dal Quadro comune europeo di riferimento per la conoscenza delle lingue (QCER), in inglese Common European Framework of Reference for Languages (CEFR).</rdfs:comment>
        <rdfs:comment xml:lang="en">This class represents the six levels (A1, A2, B1, B2, C1, C2) provided for by the Common European Framework of Reference for Languages (CEFR).</rdfs:comment>
        <rdfs:isDefinedBy rdf:resource="https://w3id.org/ecodigit/ontology/eas/"/>
        <rdfs:label xml:lang="en">CERF Level</rdfs:label>
        <rdfs:label xml:lang="it">Livello QCER (CERF)</rdfs:label>
        <owl:versionInfo xml:lang="it">stabile</owl:versionInfo>
        <owl:versionInfo xml:lang="en">stable</owl:versionInfo>
    </owl:Class>
    


    <!-- https://w3id.org/ecodigit/ontology/eas/Certification -->

    <owl:Class rdf:about="https://w3id.org/ecodigit/ontology/eas/Certification">
        <rdfs:subClassOf rdf:resource="https://w3id.org/italia/onto/l0/Object"/>
        <rdfs:subClassOf>
            <owl:Restriction>
                <owl:onProperty rdf:resource="https://w3id.org/ecodigit/ontology/eas/attests"/>
                <owl:allValuesFrom rdf:resource="https://w3id.org/italia/onto/l0/Characteristic"/>
            </owl:Restriction>
        </rdfs:subClassOf>
        <rdfs:subClassOf>
            <owl:Restriction>
                <owl:onProperty rdf:resource="https://w3id.org/ecodigit/ontology/eas/issueDate"/>
                <owl:allValuesFrom rdf:resource="http://www.w3.org/2001/XMLSchema#date"/>
            </owl:Restriction>
        </rdfs:subClassOf>
        <rdfs:comment xml:lang="it">Questa classe rappresenta la documentazione, che può essere istituzionale o autodichiarata, relativa alla Certificazione del Livello di una certa Competenza di una persona.</rdfs:comment>
        <rdfs:comment xml:lang="en">This class represents the documentation, which can be institutional or self-declared, related to the Certification of the Level of a certain Expertise of a person.</rdfs:comment>
        <rdfs:isDefinedBy rdf:resource="https://w3id.org/ecodigit/ontology/eas/"/>
        <rdfs:label xml:lang="en">Certification</rdfs:label>
        <rdfs:label>Certificazione</rdfs:label>
        <owl:versionInfo xml:lang="it">stabile</owl:versionInfo>
        <owl:versionInfo xml:lang="en">stable</owl:versionInfo>
    </owl:Class>
    


    <!-- https://w3id.org/ecodigit/ontology/eas/CertifiedExpertiseLevel -->

    <owl:Class rdf:about="https://w3id.org/ecodigit/ontology/eas/CertifiedExpertiseLevel">
        <rdfs:subClassOf rdf:resource="https://w3id.org/italia/onto/l0/Characteristic"/>
        <rdfs:comment xml:lang="it">Questa classe rappresenta il Livello di competenza attestato da una Certificazione.</rdfs:comment>
        <rdfs:comment xml:lang="en">This class represents the Level of Expertise attested by a Certification.</rdfs:comment>
        <rdfs:isDefinedBy rdf:resource="https://w3id.org/ecodigit/ontology/eas/"/>
        <rdfs:label xml:lang="en">Certified Expertise Level</rdfs:label>
        <rdfs:label xml:lang="it">Livello di competenza certificato</rdfs:label>
        <owl:versionInfo xml:lang="it">stabile</owl:versionInfo>
        <owl:versionInfo xml:lang="en">stable</owl:versionInfo>
        <prov:wasInfluencedBy rdf:resource="http://www.bbc.co.uk/ontologies/curriculum/Level"/>
    </owl:Class>
    


    <!-- https://w3id.org/ecodigit/ontology/eas/Examination -->

    <owl:Class rdf:about="https://w3id.org/ecodigit/ontology/eas/Examination">
        <rdfs:subClassOf rdf:resource="https://w3id.org/italia/onto/TI/TimeIndexedEvent"/>
        <rdfs:subClassOf>
            <owl:Restriction>
                <owl:onProperty rdf:resource="https://w3id.org/ecodigit/ontology/eas/leadsTo"/>
                <owl:someValuesFrom rdf:resource="https://w3id.org/ecodigit/ontology/eas/Certification"/>
            </owl:Restriction>
        </rdfs:subClassOf>
        <rdfs:subClassOf>
            <owl:Restriction>
                <owl:onProperty rdf:resource="https://w3id.org/ecodigit/ontology/grade/hasGrade"/>
                <owl:someValuesFrom rdf:resource="https://w3id.org/ecodigit/ontology/grade/Grade"/>
            </owl:Restriction>
        </rdfs:subClassOf>
        <rdfs:subClassOf>
            <owl:Restriction>
                <owl:onProperty rdf:resource="https://w3id.org/ecodigit/ontology/eas/hasTrainingOutcome"/>
                <owl:allValuesFrom rdf:resource="http://purl.org/ontology/bibo/Thesis"/>
            </owl:Restriction>
        </rdfs:subClassOf>
        <rdfs:comment xml:lang="it">Questa classe rappresenta la situazione di Esame, che accerta la preparazione della Persona che ha seguito l&apos;Esperienza formativa, portando al conseguimento di una Certificazione.</rdfs:comment>
        <rdfs:comment xml:lang="en">This class represents the situation of an Examination, which aims to verify the preparation of the Person who followed the Training experience, leading to the achievement of a Certification.</rdfs:comment>
        <rdfs:isDefinedBy rdf:resource="https://w3id.org/ecodigit/ontology/eas/"/>
        <rdfs:label xml:lang="it">Esame</rdfs:label>
        <rdfs:label xml:lang="en">Examination</rdfs:label>
        <owl:versionInfo xml:lang="it">stabile</owl:versionInfo>
        <owl:versionInfo xml:lang="en">stable</owl:versionInfo>
    </owl:Class>
    


    <!-- https://w3id.org/ecodigit/ontology/eas/Expertise -->

    <owl:Class rdf:about="https://w3id.org/ecodigit/ontology/eas/Expertise">
        <rdfs:subClassOf rdf:resource="https://w3id.org/italia/onto/l0/Characteristic"/>
        <rdfs:subClassOf>
            <owl:Restriction>
                <owl:onProperty rdf:resource="https://w3id.org/ecodigit/ontology/eas/hasCertification"/>
                <owl:someValuesFrom>
                    <owl:Class>
                        <owl:unionOf rdf:parseType="Collection">
                            <rdf:Description rdf:about="https://w3id.org/ecodigit/ontology/eas/IstitutionalCertification"/>
                            <rdf:Description rdf:about="https://w3id.org/ecodigit/ontology/eas/SelfCertification"/>
                        </owl:unionOf>
                    </owl:Class>
                </owl:someValuesFrom>
            </owl:Restriction>
        </rdfs:subClassOf>
        <rdfs:comment xml:lang="it">Questa classe rappresenta la competenza che una persona ha acquisito grazie a un&apos;esperienza formativa, che può essere certificata o meno.</rdfs:comment>
        <rdfs:comment xml:lang="en">This class represents the Expertise gained by a Person thanks to a Training, which may be certified or not.</rdfs:comment>
        <rdfs:isDefinedBy rdf:resource="https://w3id.org/ecodigit/ontology/eas/"/>
        <rdfs:label xml:lang="it">Competenza</rdfs:label>
        <rdfs:label xml:lang="en">Expertise</rdfs:label>
        <owl:versionInfo xml:lang="it">stabile</owl:versionInfo>
        <owl:versionInfo xml:lang="en">stable</owl:versionInfo>
        <prov:wasInfluencedBy rdf:resource="https://www.eurocris.org/ontologies/cerif/#ExpSkill"/>
    </owl:Class>
    


    <!-- https://w3id.org/ecodigit/ontology/eas/FinalExamination -->

    <owl:Class rdf:about="https://w3id.org/ecodigit/ontology/eas/FinalExamination">
        <rdfs:subClassOf rdf:resource="https://w3id.org/ecodigit/ontology/eas/Examination"/>
        <rdfs:comment xml:lang="it">Questa classe rappresenta un Esame previsto al termine di un&apos;Esperienza formativa che permette di ottenere una Certificazione. Tale Esame può avere come risultato la preparazione di una Tesi.</rdfs:comment>
        <rdfs:comment xml:lang="en">This class represents an Examination scheduled at the end of a Training experience that leads to a Certification. This Examination may result in the preparation of a Thesis.</rdfs:comment>
        <rdfs:label xml:lang="it">Esame Finale</rdfs:label>
        <rdfs:label xml:lang="en">Final Examination</rdfs:label>
        <owl:versionInfo xml:lang="it">instabile</owl:versionInfo>
        <owl:versionInfo xml:lang="en">unstable</owl:versionInfo>
    </owl:Class>
    


    <!-- https://w3id.org/ecodigit/ontology/eas/IstitutionalCertification -->

    <owl:Class rdf:about="https://w3id.org/ecodigit/ontology/eas/IstitutionalCertification">
        <rdfs:subClassOf rdf:resource="https://w3id.org/ecodigit/ontology/eas/Certification"/>
        <rdfs:subClassOf>
            <owl:Restriction>
                <owl:onProperty rdf:resource="https://w3id.org/ecodigit/ontology/eas/issuedBy"/>
                <owl:someValuesFrom rdf:resource="https://w3id.org/italia/onto/COV/Organization"/>
            </owl:Restriction>
        </rdfs:subClassOf>
        <owl:disjointWith rdf:resource="https://w3id.org/ecodigit/ontology/eas/SelfCertification"/>
        <rdfs:comment xml:lang="it">Questa classe rappresenta le Certificazioni emesse ufficialmente da una Organizzazione.</rdfs:comment>
        <rdfs:comment xml:lang="en">This class represents the Certifications officially issued by an Organization.</rdfs:comment>
        <rdfs:isDefinedBy rdf:resource="https://w3id.org/ecodigit/ontology/eas/"/>
        <rdfs:label xml:lang="it">Certificazione istituzionale</rdfs:label>
        <rdfs:label xml:lang="en">Istitutional Certification</rdfs:label>
        <owl:versionInfo xml:lang="it">stabile</owl:versionInfo>
        <owl:versionInfo xml:lang="en">stable</owl:versionInfo>
    </owl:Class>
    


    <!-- https://w3id.org/ecodigit/ontology/eas/LanguageActivity -->

    <owl:Class rdf:about="https://w3id.org/ecodigit/ontology/eas/LanguageActivity">
        <rdfs:subClassOf rdf:resource="https://w3id.org/italia/onto/l0/Activity"/>
        <rdfs:comment xml:lang="it">Questa classe rappresenta i vari tipi di attività linguistiche (ad es. comprensione scritta, produzione orale, ecc.).</rdfs:comment>
        <rdfs:comment xml:lang="en">This class represents the various types of language activities (e.g. written comprehension, spoken interaction, etc.).</rdfs:comment>
        <rdfs:isDefinedBy rdf:resource="https://w3id.org/ecodigit/ontology/eas/"/>
        <rdfs:label xml:lang="it">Attività linguistica</rdfs:label>
        <rdfs:label xml:lang="en">Language activity</rdfs:label>
        <owl:versionInfo xml:lang="it">stabile</owl:versionInfo>
        <owl:versionInfo xml:lang="en">stable</owl:versionInfo>
    </owl:Class>
    


    <!-- https://w3id.org/ecodigit/ontology/eas/LanguageSkill -->

    <owl:Class rdf:about="https://w3id.org/ecodigit/ontology/eas/LanguageSkill">
        <rdfs:subClassOf rdf:resource="https://w3id.org/ecodigit/ontology/eas/Expertise"/>
        <rdfs:subClassOf>
            <owl:Restriction>
                <owl:onProperty rdf:resource="https://w3id.org/italia/onto/Language/hasLanguage"/>
                <owl:someValuesFrom rdf:resource="https://w3id.org/italia/onto/Language/Language"/>
            </owl:Restriction>
        </rdfs:subClassOf>
        <rdfs:comment xml:lang="it">Questa classe rappresenta l&apos;abilità linguistica che una persona ha acquisito grazie a un&apos;esperienza formativa, che può essere certificata o meno.</rdfs:comment>
        <rdfs:comment xml:lang="en">This class represents the Language skill gained by a Person thanks to a Training, which may be certified or not.</rdfs:comment>
        <rdfs:isDefinedBy rdf:resource="https://w3id.org/ecodigit/ontology/eas/"/>
        <rdfs:label xml:lang="it">Abilità linguistiche</rdfs:label>
        <rdfs:label xml:lang="en">Language skill</rdfs:label>
        <owl:versionInfo xml:lang="it">stabile</owl:versionInfo>
        <owl:versionInfo xml:lang="en">stable</owl:versionInfo>
    </owl:Class>
    


    <!-- https://w3id.org/ecodigit/ontology/eas/LevelInActivity -->

    <owl:Class rdf:about="https://w3id.org/ecodigit/ontology/eas/LevelInActivity">
        <rdfs:subClassOf rdf:resource="https://w3id.org/italia/onto/l0/Characteristic"/>
        <rdfs:subClassOf>
            <owl:Restriction>
                <owl:onProperty rdf:resource="https://w3id.org/ecodigit/ontology/eas/hasActivity"/>
                <owl:someValuesFrom rdf:resource="https://w3id.org/italia/onto/l0/Activity"/>
            </owl:Restriction>
        </rdfs:subClassOf>
        <rdfs:subClassOf>
            <owl:Restriction>
                <owl:onProperty rdf:resource="https://w3id.org/ecodigit/ontology/eas/hasCertifiedExpertiseLevel"/>
                <owl:someValuesFrom rdf:resource="https://w3id.org/ecodigit/ontology/eas/CertifiedExpertiseLevel"/>
            </owl:Restriction>
        </rdfs:subClassOf>
        <rdfs:comment xml:lang="it">Questa classe rappresenta il Livello attestato da un Certificato in una certa Attività. Questa classe è una reificazione della proprietà &apos;eas:attests&apos;. La classe permette di specificare oltre al livello attestato una eventuale attività a cui si riferisce il livello. La modellazione di questa classe è influenzata dal Common European Framework of Reference for Languages (CERF). In CERF è possibile esprimere il fatto che una persona ha raggiunto un certo livello (e.g. B1) in una attività del linguaggio (e.g. Listening Comprehension) e un altro livello (e.g. C1) in un&apos;altra attività del linguaggio (e.g. Reading Compehension).</rdfs:comment>
        <rdfs:comment xml:lang="en">This class represents the Level attested by a Certification in a certain Activity. This class is a reification of the &apos;eas: attests&apos; property. In addition to the Certified expertise level, this class allows to specify any activity to which the level refers. The modeling of this class is influenced by the Common European Framework of Reference for Languages (CERF). In CERF it is possible to express the fact that a person has reached a certain level (e.g. B1) in certain language activity (e.g. Listening Comprehension) and another level (e.g. C1) in another language activity (e.g. Reading Compehension).</rdfs:comment>
        <rdfs:isDefinedBy rdf:resource="https://w3id.org/ecodigit/ontology/eas/"/>
        <rdfs:label xml:lang="en">Level in Activity</rdfs:label>
        <rdfs:label xml:lang="it">Livello in Attività</rdfs:label>
        <owl:versionInfo xml:lang="it">stabile</owl:versionInfo>
        <owl:versionInfo xml:lang="en">stable</owl:versionInfo>
    </owl:Class>
    


    <!-- https://w3id.org/ecodigit/ontology/eas/SelfCertification -->

    <owl:Class rdf:about="https://w3id.org/ecodigit/ontology/eas/SelfCertification">
        <rdfs:subClassOf rdf:resource="https://w3id.org/ecodigit/ontology/eas/Certification"/>
        <rdfs:comment xml:lang="it">Questa classe rappresenta le Autocertificazioni redatte da una Persona sotto la propria responsabilità a norma di legge.</rdfs:comment>
        <rdfs:comment xml:lang="en">This class represents the Self-certifications drawn up by a Person under his own responsibility according to the law.</rdfs:comment>
        <rdfs:isDefinedBy rdf:resource="https://w3id.org/ecodigit/ontology/eas/"/>
        <rdfs:label xml:lang="it">Autocertificazione</rdfs:label>
        <rdfs:label xml:lang="en">Self-certification</rdfs:label>
        <owl:versionInfo xml:lang="it">stabile</owl:versionInfo>
        <owl:versionInfo xml:lang="en">stable</owl:versionInfo>
    </owl:Class>
    


    <!-- https://w3id.org/ecodigit/ontology/eas/Training -->

    <owl:Class rdf:about="https://w3id.org/ecodigit/ontology/eas/Training">
        <rdfs:subClassOf rdf:resource="https://w3id.org/italia/onto/TI/TimeIndexedEvent"/>
        <rdfs:subClassOf>
            <owl:Restriction>
                <owl:onProperty rdf:resource="https://w3id.org/ecodigit/ontology/eas/isAttendedBy"/>
                <owl:someValuesFrom rdf:resource="https://w3id.org/italia/onto/CPV/Person"/>
            </owl:Restriction>
        </rdfs:subClassOf>
        <rdfs:subClassOf>
            <owl:Restriction>
                <owl:onProperty rdf:resource="https://w3id.org/ecodigit/ontology/eas/providedBy"/>
                <owl:someValuesFrom rdf:resource="https://w3id.org/italia/onto/COV/Organization"/>
            </owl:Restriction>
        </rdfs:subClassOf>
        <rdfs:subClassOf>
            <owl:Restriction>
                <owl:onProperty rdf:resource="https://w3id.org/ecodigit/ontology/eas/hasCertification"/>
                <owl:allValuesFrom rdf:resource="https://w3id.org/ecodigit/ontology/eas/Certification"/>
            </owl:Restriction>
        </rdfs:subClassOf>
        <rdfs:subClassOf>
            <owl:Restriction>
                <owl:onProperty rdf:resource="https://w3id.org/ecodigit/ontology/eas/includesAnExamination"/>
                <owl:allValuesFrom rdf:resource="https://w3id.org/ecodigit/ontology/eas/Examination"/>
            </owl:Restriction>
        </rdfs:subClassOf>
        <rdfs:comment xml:lang="it">La classe rappresenta le Esperienze formative, erogate da una Organizzazione, a cui una Persona ha partecipato. Esse possono prevedere o meno un Esame con relativa Certificazione.</rdfs:comment>
        <rdfs:comment xml:lang="en">The class represents the Training experiences, provided by an Organization and attended by a Person. They may include or not an Examination with a Certification.</rdfs:comment>
        <rdfs:isDefinedBy rdf:resource="https://w3id.org/ecodigit/ontology/eas/"/>
        <rdfs:label xml:lang="it">Esperienza Formativa</rdfs:label>
        <rdfs:label xml:lang="en">Training</rdfs:label>
        <owl:versionInfo xml:lang="it">stabile</owl:versionInfo>
        <owl:versionInfo xml:lang="en">stable</owl:versionInfo>
    </owl:Class>
    


    <!-- https://w3id.org/italia/onto/COV/Organization -->

    <owl:Class rdf:about="https://w3id.org/italia/onto/COV/Organization"/>
    


    <!-- https://w3id.org/italia/onto/l0/Activity -->

    <owl:Class rdf:about="https://w3id.org/italia/onto/l0/Activity"/>
    


    <!-- 
    ///////////////////////////////////////////////////////////////////////////////////////
    //
    // Individuals
    //
    ///////////////////////////////////////////////////////////////////////////////////////
     -->

    


    <!-- https://w3id.org/ecodigit/ontology/eas/A1 -->

    <owl:NamedIndividual rdf:about="https://w3id.org/ecodigit/ontology/eas/A1">
        <rdf:type rdf:resource="https://w3id.org/ecodigit/ontology/eas/CERFLevel"/>
        <rdfs:comment xml:lang="it">Questo individuo rappresenta il livello base A1 del Common European Framework of Reference for Languages (CEFR).</rdfs:comment>
        <rdfs:comment xml:lang="en">This individual represents the A1 beginner level of the Common European Framework of Reference for Languages ​​(CEFR).</rdfs:comment>
        <rdfs:isDefinedBy rdf:resource="https://w3id.org/ecodigit/ontology/eas/"/>
        <rdfs:label xml:lang="en">Level A1</rdfs:label>
        <rdfs:label xml:lang="it">Livello A1</rdfs:label>
        <owl:versionInfo xml:lang="it">stabile</owl:versionInfo>
        <owl:versionInfo xml:lang="en">stable</owl:versionInfo>
    </owl:NamedIndividual>
    


    <!-- https://w3id.org/ecodigit/ontology/eas/A2 -->

    <owl:NamedIndividual rdf:about="https://w3id.org/ecodigit/ontology/eas/A2">
        <rdf:type rdf:resource="https://w3id.org/ecodigit/ontology/eas/CERFLevel"/>
        <rdfs:comment xml:lang="it">Questo individuo rappresenta il livello elementare A2 del Common European Framework of Reference for Languages (CEFR).</rdfs:comment>
        <rdfs:comment xml:lang="en">This individual represents the A2 elementary level of the Common European Framework of Reference for Languages ​​(CEFR).</rdfs:comment>
        <rdfs:isDefinedBy rdf:resource="https://w3id.org/ecodigit/ontology/eas/"/>
        <rdfs:label xml:lang="en">Level A2</rdfs:label>
        <rdfs:label xml:lang="it">Livello A2</rdfs:label>
        <owl:versionInfo xml:lang="it">stabile</owl:versionInfo>
        <owl:versionInfo xml:lang="en">stable</owl:versionInfo>
    </owl:NamedIndividual>
    


    <!-- https://w3id.org/ecodigit/ontology/eas/B1 -->

    <owl:NamedIndividual rdf:about="https://w3id.org/ecodigit/ontology/eas/B1">
        <rdf:type rdf:resource="https://w3id.org/ecodigit/ontology/eas/CERFLevel"/>
        <rdfs:comment xml:lang="it">Questo individuo rappresenta il livello intermedio B1 del Common European Framework of Reference for Languages (CEFR).</rdfs:comment>
        <rdfs:comment xml:lang="en">This individual represents the B1 intermediate level of the Common European Framework of Reference for Languages ​​(CEFR).</rdfs:comment>
        <rdfs:isDefinedBy rdf:resource="https://w3id.org/ecodigit/ontology/eas/"/>
        <rdfs:label xml:lang="en">Level B1</rdfs:label>
        <rdfs:label xml:lang="it">Livello B1</rdfs:label>
        <owl:versionInfo xml:lang="it">stabile</owl:versionInfo>
        <owl:versionInfo xml:lang="en">stable</owl:versionInfo>
    </owl:NamedIndividual>
    


    <!-- https://w3id.org/ecodigit/ontology/eas/B2 -->

    <owl:NamedIndividual rdf:about="https://w3id.org/ecodigit/ontology/eas/B2">
        <rdf:type rdf:resource="https://w3id.org/ecodigit/ontology/eas/CERFLevel"/>
        <rdfs:comment xml:lang="it">Questo individuo rappresenta il livello intermedio superiore B2 del Common European Framework of Reference for Languages (CEFR).</rdfs:comment>
        <rdfs:comment xml:lang="en">This individual represents the B2 upper intermediate level of the Common European Framework of Reference for Languages ​​(CEFR).</rdfs:comment>
        <rdfs:isDefinedBy rdf:resource="https://w3id.org/ecodigit/ontology/eas/"/>
        <rdfs:label xml:lang="en">Level B2</rdfs:label>
        <rdfs:label xml:lang="it">Livello B2</rdfs:label>
        <owl:versionInfo xml:lang="it">stabile</owl:versionInfo>
        <owl:versionInfo xml:lang="en">stable</owl:versionInfo>
    </owl:NamedIndividual>
    


    <!-- https://w3id.org/ecodigit/ontology/eas/C1 -->

    <owl:NamedIndividual rdf:about="https://w3id.org/ecodigit/ontology/eas/C1">
        <rdf:type rdf:resource="https://w3id.org/ecodigit/ontology/eas/CERFLevel"/>
        <rdfs:comment xml:lang="it">Questo individuo rappresenta il livello avanzato C1 del Common European Framework of Reference for Languages (CEFR).</rdfs:comment>
        <rdfs:comment xml:lang="en">This individual represents the C1 advanced level of the Common European Framework of Reference for Languages ​​(CEFR).</rdfs:comment>
        <rdfs:isDefinedBy rdf:resource="https://w3id.org/ecodigit/ontology/eas/"/>
        <rdfs:label xml:lang="en">Level C1</rdfs:label>
        <rdfs:label xml:lang="it">Livello C1</rdfs:label>
        <owl:versionInfo xml:lang="it">stabile</owl:versionInfo>
        <owl:versionInfo xml:lang="en">stable</owl:versionInfo>
    </owl:NamedIndividual>
    


    <!-- https://w3id.org/ecodigit/ontology/eas/C2 -->

    <owl:NamedIndividual rdf:about="https://w3id.org/ecodigit/ontology/eas/C2">
        <rdf:type rdf:resource="https://w3id.org/ecodigit/ontology/eas/CERFLevel"/>
        <rdfs:comment xml:lang="it">Questo individuo rappresenta il livello di padronanza C2 del Common European Framework of Reference for Languages (CEFR).</rdfs:comment>
        <rdfs:comment xml:lang="en">This individual represents the C2 proficiency level of the Common European Framework of Reference for Languages ​​(CEFR).</rdfs:comment>
        <rdfs:isDefinedBy rdf:resource="https://w3id.org/ecodigit/ontology/eas/"/>
        <rdfs:label xml:lang="en">Level C2</rdfs:label>
        <rdfs:label xml:lang="it">Livello C2</rdfs:label>
        <owl:versionInfo xml:lang="it">stabile</owl:versionInfo>
        <owl:versionInfo xml:lang="en">stable</owl:versionInfo>
    </owl:NamedIndividual>
    


    <!-- https://w3id.org/ecodigit/ontology/eas/Interaction -->

    <owl:NamedIndividual rdf:about="https://w3id.org/ecodigit/ontology/eas/Interaction">
        <rdf:type rdf:resource="https://w3id.org/ecodigit/ontology/eas/LanguageActivity"/>
        <rdfs:isDefinedBy rdf:resource="https://w3id.org/ecodigit/ontology/eas/"/>
        <rdfs:label xml:lang="en">Interaction</rdfs:label>
        <rdfs:label xml:lang="it">Interazione</rdfs:label>
        <owl:versionInfo xml:lang="it">stabile</owl:versionInfo>
        <owl:versionInfo xml:lang="en">stable</owl:versionInfo>
    </owl:NamedIndividual>
    


    <!-- https://w3id.org/ecodigit/ontology/eas/ListeningComprehension -->

    <owl:NamedIndividual rdf:about="https://w3id.org/ecodigit/ontology/eas/ListeningComprehension">
        <rdf:type rdf:resource="https://w3id.org/ecodigit/ontology/eas/LanguageActivity"/>
        <rdfs:isDefinedBy rdf:resource="https://w3id.org/ecodigit/ontology/eas/"/>
        <rdfs:label xml:lang="it">Comprensione orale</rdfs:label>
        <rdfs:label xml:lang="en">Listening comprehension</rdfs:label>
        <owl:versionInfo xml:lang="it">stabile</owl:versionInfo>
        <owl:versionInfo xml:lang="en">stable</owl:versionInfo>
    </owl:NamedIndividual>
    


    <!-- https://w3id.org/ecodigit/ontology/eas/Production -->

    <owl:NamedIndividual rdf:about="https://w3id.org/ecodigit/ontology/eas/Production">
        <rdf:type rdf:resource="https://w3id.org/ecodigit/ontology/eas/LanguageActivity"/>
        <rdfs:isDefinedBy rdf:resource="https://w3id.org/ecodigit/ontology/eas/"/>
        <rdfs:label xml:lang="en">Production</rdfs:label>
        <rdfs:label xml:lang="it">Produzione</rdfs:label>
        <owl:versionInfo xml:lang="it">stabile</owl:versionInfo>
        <owl:versionInfo xml:lang="en">stable</owl:versionInfo>
    </owl:NamedIndividual>
    


    <!-- https://w3id.org/ecodigit/ontology/eas/ReadingComprehension -->

    <owl:NamedIndividual rdf:about="https://w3id.org/ecodigit/ontology/eas/ReadingComprehension">
        <rdf:type rdf:resource="https://w3id.org/ecodigit/ontology/eas/LanguageActivity"/>
        <rdfs:isDefinedBy rdf:resource="https://w3id.org/ecodigit/ontology/eas/"/>
        <rdfs:label xml:lang="it">Comprensione scritta</rdfs:label>
        <rdfs:label xml:lang="en">Reading comprehension</rdfs:label>
        <owl:versionInfo xml:lang="it">stabile</owl:versionInfo>
        <owl:versionInfo xml:lang="en">stable</owl:versionInfo>
    </owl:NamedIndividual>
    


    <!-- https://w3id.org/ecodigit/ontology/eas/Reception -->

    <owl:NamedIndividual rdf:about="https://w3id.org/ecodigit/ontology/eas/Reception">
        <rdf:type rdf:resource="https://w3id.org/ecodigit/ontology/eas/LanguageActivity"/>
    </owl:NamedIndividual>
    


    <!-- https://w3id.org/ecodigit/ontology/eas/SpokenInteraction -->

    <owl:NamedIndividual rdf:about="https://w3id.org/ecodigit/ontology/eas/SpokenInteraction">
        <rdf:type rdf:resource="https://w3id.org/ecodigit/ontology/eas/LanguageActivity"/>
        <rdfs:isDefinedBy rdf:resource="https://w3id.org/ecodigit/ontology/eas/"/>
        <rdfs:label xml:lang="it">Interazione parlata</rdfs:label>
        <rdfs:label xml:lang="en">Spoken interaction</rdfs:label>
        <owl:versionInfo xml:lang="it">stabile</owl:versionInfo>
        <owl:versionInfo xml:lang="en">stable</owl:versionInfo>
    </owl:NamedIndividual>
    


    <!-- https://w3id.org/ecodigit/ontology/eas/SpokenProduction -->

    <owl:NamedIndividual rdf:about="https://w3id.org/ecodigit/ontology/eas/SpokenProduction">
        <rdf:type rdf:resource="https://w3id.org/ecodigit/ontology/eas/LanguageActivity"/>
        <rdfs:isDefinedBy rdf:resource="https://w3id.org/ecodigit/ontology/eas/"/>
        <rdfs:label xml:lang="it">Produzione parlata</rdfs:label>
        <rdfs:label xml:lang="en">Spoken production</rdfs:label>
        <owl:versionInfo xml:lang="it">stabile</owl:versionInfo>
        <owl:versionInfo xml:lang="en">stable</owl:versionInfo>
    </owl:NamedIndividual>
    


    <!-- https://w3id.org/ecodigit/ontology/eas/WrittenInteraction -->

    <owl:NamedIndividual rdf:about="https://w3id.org/ecodigit/ontology/eas/WrittenInteraction">
        <rdf:type rdf:resource="https://w3id.org/ecodigit/ontology/eas/LanguageActivity"/>
        <rdfs:isDefinedBy rdf:resource="https://w3id.org/ecodigit/ontology/eas/"/>
        <rdfs:label xml:lang="it">Interazione scritta</rdfs:label>
        <rdfs:label xml:lang="en">Written interaction</rdfs:label>
        <owl:versionInfo xml:lang="it">stabile</owl:versionInfo>
        <owl:versionInfo xml:lang="en">stable</owl:versionInfo>
    </owl:NamedIndividual>
    


    <!-- https://w3id.org/ecodigit/ontology/eas/WrittenProduction -->

    <owl:NamedIndividual rdf:about="https://w3id.org/ecodigit/ontology/eas/WrittenProduction">
        <rdf:type rdf:resource="https://w3id.org/ecodigit/ontology/eas/LanguageActivity"/>
        <rdfs:isDefinedBy rdf:resource="https://w3id.org/ecodigit/ontology/eas/"/>
        <rdfs:label xml:lang="it">Produzione scritta</rdfs:label>
        <rdfs:label xml:lang="en">Written production</rdfs:label>
        <owl:versionInfo xml:lang="it">stabile</owl:versionInfo>
        <owl:versionInfo xml:lang="en">stable</owl:versionInfo>
    </owl:NamedIndividual>
</rdf:RDF>



<!-- Generated by the OWL API (version 4.5.9.2019-02-01T07:24:44Z) https://github.com/owlcs/owlapi -->

