<?xml version="1.0"?>
<rdf:RDF xmlns="https://w3id.org/ecodigit/ontology/eas/"
     xml:base="https://w3id.org/ecodigit/ontology/eas/"
     xmlns:dc="http://purl.org/dc/elements/1.1/"
     xmlns:l0="https://w3id.org/italia/onto/l0/"
     xmlns:ns="http://www.w3.org/2003/06/sw-vocab-status/ns#"
     xmlns:CLV="https://w3id.org/italia/onto/CLV/"
     xmlns:ns1="http://www.w3.org/2006/vcard/ns#"
     xmlns:owl="http://www.w3.org/2002/07/owl#"
     xmlns:rdf="http://www.w3.org/1999/02/22-rdf-syntax-ns#"
     xmlns:wot="http://xmlns.com/wot/0.1/"
     xmlns:xml="http://www.w3.org/XML/1998/namespace"
     xmlns:xsd="http://www.w3.org/2001/XMLSchema#"
     xmlns:ADMS="https://w3id.org/italia/onto/ADMS/"
     xmlns:dcat="http://www.w3.org/ns/dcat#"
     xmlns:foaf="http://xmlns.com/foaf/0.1/"
     xmlns:prov="http://www.w3.org/ns/prov#"
     xmlns:rdfs="http://www.w3.org/2000/01/rdf-schema#"
     xmlns:skos="http://www.w3.org/2004/02/skos/core#"
     xmlns:terms="http://purl.org/dc/terms/"
     xmlns:ecodigit-eas="https://w3id.org/ecodigit/ontology/eas/">
    <owl:Ontology rdf:about="https://w3id.org/ecodigit/ontology/eas/">
        <owl:versionIRI rdf:resource="https://w3id.org/ecodigit/ontology/eas/0.1/"/>
        <owl:imports rdf:resource="http://purl.org/ontology/bibo/"/>
        <owl:imports rdf:resource="http://xmlns.com/foaf/0.1/"/>
        <owl:imports rdf:resource="https://w3id.org/ecodigit/ontology/grade"/>
        <owl:imports rdf:resource="https://w3id.org/italia/onto/COV"/>
        <owl:imports rdf:resource="https://w3id.org/italia/onto/CPV"/>
        <owl:imports rdf:resource="https://w3id.org/italia/onto/Language"/>
    </owl:Ontology>
    


    <!-- 
    ///////////////////////////////////////////////////////////////////////////////////////
    //
    // Object Properties
    //
    ///////////////////////////////////////////////////////////////////////////////////////
     -->

    


    <!-- https://w3id.org/ecodigit/ontology/eas/attends -->

    <owl:ObjectProperty rdf:about="https://w3id.org/ecodigit/ontology/eas/attends">
        <owl:inverseOf rdf:resource="https://w3id.org/ecodigit/ontology/eas/isAttendedBy"/>
        <rdfs:domain rdf:resource="https://w3id.org/italia/onto/CPV/Person"/>
        <rdfs:range rdf:resource="https://w3id.org/ecodigit/ontology/eas/Training"/>
        <rdfs:comment xml:lang="it">Questa proprietà permette di associare una Persona con l&apos;Esperienza formativa da essa frequentata.</rdfs:comment>
        <rdfs:comment xml:lang="en">This property associates a Person with the attended Training.</rdfs:comment>
        <rdfs:label xml:lang="en">attends</rdfs:label>
        <rdfs:label xml:lang="it">frequenta</rdfs:label>
        <owl:versionInfo xml:lang="it">instabile</owl:versionInfo>
        <owl:versionInfo xml:lang="en">unstable</owl:versionInfo>
    </owl:ObjectProperty>
    


    <!-- https://w3id.org/ecodigit/ontology/eas/attests -->

    <owl:ObjectProperty rdf:about="https://w3id.org/ecodigit/ontology/eas/attests">
        <owl:inverseOf rdf:resource="https://w3id.org/ecodigit/ontology/eas/isAttestedBy"/>
        <rdfs:domain rdf:resource="https://w3id.org/ecodigit/ontology/eas/Certification"/>
        <rdfs:range>
            <owl:Class>
                <owl:unionOf rdf:parseType="Collection">
                    <rdf:Description rdf:about="https://w3id.org/ecodigit/ontology/eas/Level"/>
                    <rdf:Description rdf:about="https://w3id.org/italia/onto/CPV/EducationLevel"/>
                </owl:unionOf>
            </owl:Class>
        </rdfs:range>
        <rdfs:comment xml:lang="it">Questa proprietà permette di associare una Certificazione con il Livello di istruzione o competenza attestato.</rdfs:comment>
        <rdfs:comment xml:lang="en">This property associates a Certification with the attested Level of Education or Expertise.</rdfs:comment>
        <rdfs:label xml:lang="it">attesta</rdfs:label>
        <rdfs:label xml:lang="en">attests</rdfs:label>
        <owl:versionInfo xml:lang="it">instabile</owl:versionInfo>
        <owl:versionInfo xml:lang="en">unstable</owl:versionInfo>
    </owl:ObjectProperty>
    


    <!-- https://w3id.org/ecodigit/ontology/eas/hasActivity -->

    <owl:ObjectProperty rdf:about="https://w3id.org/ecodigit/ontology/eas/hasActivity">
        <rdfs:domain rdf:resource="https://w3id.org/ecodigit/ontology/eas/LevelInActivity"/>
        <rdfs:range rdf:resource="https://w3id.org/italia/onto/l0/Activity"/>
        <rdfs:label xml:lang="it">Associa il Livello in Attività con l&apos;attività a cui si riferisce.</rdfs:label>
        <rdfs:label xml:lang="it">ha attività</rdfs:label>
        <rdfs:label xml:lang="en">has activity</rdfs:label>
        <owl:versionInfo xml:lang="en">unstable</owl:versionInfo>
    </owl:ObjectProperty>
    


    <!-- https://w3id.org/ecodigit/ontology/eas/hasCertification -->

    <owl:ObjectProperty rdf:about="https://w3id.org/ecodigit/ontology/eas/hasCertification">
        <owl:inverseOf rdf:resource="https://w3id.org/ecodigit/ontology/eas/isCertificationOf"/>
        <rdfs:domain rdf:resource="http://www.w3.org/2002/07/owl#Thing"/>
        <rdfs:range rdf:resource="https://w3id.org/ecodigit/ontology/eas/Certification"/>
        <rdfs:comment xml:lang="it">Questa proprietà associa una Entità alla sua Certificazione sia essa istituzionale o autodichiarata.</rdfs:comment>
        <rdfs:comment xml:lang="en">This property associates an Entity with its Certification whether it is institutional or self-declared.</rdfs:comment>
        <rdfs:label xml:lang="it">ha certificazione</rdfs:label>
        <rdfs:label xml:lang="en">has certification</rdfs:label>
        <owl:versionInfo xml:lang="it">instabile</owl:versionInfo>
        <owl:versionInfo xml:lang="en">unstable</owl:versionInfo>
    </owl:ObjectProperty>
    


    <!-- https://w3id.org/ecodigit/ontology/eas/hasExpertise -->

    <owl:ObjectProperty rdf:about="https://w3id.org/ecodigit/ontology/eas/hasExpertise">
        <rdfs:domain rdf:resource="http://xmlns.com/foaf/0.1/Person"/>
        <rdfs:range rdf:resource="https://w3id.org/ecodigit/ontology/eas/ExpertiseAndSkill"/>
        <rdfs:comment xml:lang="it">Questa proprietà associa una Persona con la sua Esperienza o Competenza.</rdfs:comment>
        <rdfs:comment xml:lang="en">This property associates a Person with his Expertise or Competence.</rdfs:comment>
        <rdfs:label xml:lang="it">ha esperienza</rdfs:label>
        <rdfs:label xml:lang="en">has expertise</rdfs:label>
        <owl:versionInfo xml:lang="it">instabile</owl:versionInfo>
        <owl:versionInfo xml:lang="en">unstable</owl:versionInfo>
        <prov:wasInfluencedBy rdf:resource="http://purl.org/ontology/cco/core#expertise"/>
    </owl:ObjectProperty>
    


    <!-- https://w3id.org/ecodigit/ontology/eas/hasLevel -->

    <owl:ObjectProperty rdf:about="https://w3id.org/ecodigit/ontology/eas/hasLevel">
        <rdfs:domain rdf:resource="https://w3id.org/ecodigit/ontology/eas/LevelInActivity"/>
        <rdfs:range rdf:resource="https://w3id.org/ecodigit/ontology/eas/Level"/>
        <rdfs:comment xml:lang="it">Associa un Livello in Attività con il Livello a cui si riferisce.</rdfs:comment>
        <rdfs:label xml:lang="it">ha livello</rdfs:label>
        <rdfs:label xml:lang="en">has level</rdfs:label>
        <owl:versionInfo xml:lang="en">unstable</owl:versionInfo>
    </owl:ObjectProperty>
    


    <!-- https://w3id.org/ecodigit/ontology/eas/hasTrainingOutcome -->

    <owl:ObjectProperty rdf:about="https://w3id.org/ecodigit/ontology/eas/hasTrainingOutcome">
        <owl:inverseOf rdf:resource="https://w3id.org/ecodigit/ontology/eas/isTrainingOutcomeOf"/>
        <rdfs:domain>
            <owl:Class>
                <owl:unionOf rdf:parseType="Collection">
                    <rdf:Description rdf:about="https://w3id.org/ecodigit/ontology/eas/Examination"/>
                    <rdf:Description rdf:about="https://w3id.org/ecodigit/ontology/eas/Training"/>
                </owl:unionOf>
            </owl:Class>
        </rdfs:domain>
        <rdfs:comment xml:lang="it">Questa proprietà associa un&apos;Esperienza formativa o un Esame con il Risultato della formazione, per esempio una Tesi.</rdfs:comment>
        <rdfs:comment xml:lang="en">This property associates a Training experience or an Examination with the Training outcome, e.g. a Thesis.</rdfs:comment>
        <rdfs:label xml:lang="it">ha risultato della formazione</rdfs:label>
        <rdfs:label xml:lang="en">has training outcome</rdfs:label>
        <owl:versionInfo xml:lang="it">instabile</owl:versionInfo>
        <owl:versionInfo xml:lang="en">unstable</owl:versionInfo>
    </owl:ObjectProperty>
    


    <!-- https://w3id.org/ecodigit/ontology/eas/includesAnExamination -->

    <owl:ObjectProperty rdf:about="https://w3id.org/ecodigit/ontology/eas/includesAnExamination">
        <rdfs:domain rdf:resource="https://w3id.org/ecodigit/ontology/eas/Training"/>
        <rdfs:range rdf:resource="https://w3id.org/ecodigit/ontology/eas/Examination"/>
        <rdfs:comment xml:lang="it">La proprietà permette di associare una Esperienza formativa con gli esami necessari per il suo completamento.</rdfs:comment>
        <rdfs:comment xml:lang="en">The property associates a Training with the Examinations required for its completion.</rdfs:comment>
        <rdfs:label xml:lang="it">include un esame</rdfs:label>
        <rdfs:label xml:lang="en">includes an examination</rdfs:label>
        <owl:versionInfo xml:lang="it">instabile</owl:versionInfo>
        <owl:versionInfo xml:lang="en">unstable</owl:versionInfo>
    </owl:ObjectProperty>
    


    <!-- https://w3id.org/ecodigit/ontology/eas/isAttendedBy -->

    <owl:ObjectProperty rdf:about="https://w3id.org/ecodigit/ontology/eas/isAttendedBy">
        <rdfs:domain rdf:resource="https://w3id.org/ecodigit/ontology/eas/Training"/>
        <rdfs:range rdf:resource="http://xmlns.com/foaf/0.1/Person"/>
        <rdfs:comment xml:lang="it">Questa è la proprietà inversa di &apos;frequenta&apos;.</rdfs:comment>
        <rdfs:comment xml:lang="en">This is the inverse object property of &apos;attends&apos;.</rdfs:comment>
        <rdfs:label xml:lang="en">is attended by</rdfs:label>
        <rdfs:label xml:lang="it">è frequentato da</rdfs:label>
        <owl:versionInfo xml:lang="it">instabile</owl:versionInfo>
        <owl:versionInfo xml:lang="en">unstable</owl:versionInfo>
    </owl:ObjectProperty>
    


    <!-- https://w3id.org/ecodigit/ontology/eas/isAttestedBy -->

    <owl:ObjectProperty rdf:about="https://w3id.org/ecodigit/ontology/eas/isAttestedBy">
        <rdfs:domain>
            <owl:Class>
                <owl:unionOf rdf:parseType="Collection">
                    <rdf:Description rdf:about="https://w3id.org/ecodigit/ontology/eas/Level"/>
                    <rdf:Description rdf:about="https://w3id.org/italia/onto/CPV/EducationLevel"/>
                </owl:unionOf>
            </owl:Class>
        </rdfs:domain>
        <rdfs:range rdf:resource="https://w3id.org/ecodigit/ontology/eas/Certification"/>
        <rdfs:comment xml:lang="it">Questa è la proprietà inversa di &apos;attesta&apos;.</rdfs:comment>
        <rdfs:comment xml:lang="en">This is the inverse object property of &apos;attests&apos;.</rdfs:comment>
        <rdfs:label xml:lang="en">is attested by</rdfs:label>
        <rdfs:label xml:lang="it">è attestato da</rdfs:label>
        <owl:versionInfo xml:lang="it">instabile</owl:versionInfo>
        <owl:versionInfo xml:lang="en">unstable</owl:versionInfo>
    </owl:ObjectProperty>
    


    <!-- https://w3id.org/ecodigit/ontology/eas/isCertificationOf -->

    <owl:ObjectProperty rdf:about="https://w3id.org/ecodigit/ontology/eas/isCertificationOf">
        <rdfs:domain rdf:resource="https://w3id.org/ecodigit/ontology/eas/Certification"/>
        <rdfs:range rdf:resource="http://www.w3.org/2002/07/owl#Thing"/>
        <rdfs:comment xml:lang="it">Questa è la proprietà inversa di &apos;ha certificazione&apos;.</rdfs:comment>
        <rdfs:comment xml:lang="en">This is the inverse object property of &apos;has certification&apos;.</rdfs:comment>
        <rdfs:label xml:lang="en">is certification of</rdfs:label>
        <rdfs:label xml:lang="it">è certificazione di</rdfs:label>
        <owl:versionInfo xml:lang="it">instabile</owl:versionInfo>
        <owl:versionInfo xml:lang="it">unstable</owl:versionInfo>
    </owl:ObjectProperty>
    


    <!-- https://w3id.org/ecodigit/ontology/eas/isTrainingOutcomeOf -->

    <owl:ObjectProperty rdf:about="https://w3id.org/ecodigit/ontology/eas/isTrainingOutcomeOf">
        <rdfs:range>
            <owl:Class>
                <owl:unionOf rdf:parseType="Collection">
                    <rdf:Description rdf:about="https://w3id.org/ecodigit/ontology/eas/Examination"/>
                    <rdf:Description rdf:about="https://w3id.org/ecodigit/ontology/eas/Training"/>
                </owl:unionOf>
            </owl:Class>
        </rdfs:range>
        <rdfs:comment xml:lang="it">Questa è la proprietà inversa di &apos;ha risultato della formazione&apos;.</rdfs:comment>
        <rdfs:comment xml:lang="en">This is the inverse object property of &apos;has training outcome&apos;.</rdfs:comment>
        <rdfs:label xml:lang="en">is training outcome of</rdfs:label>
        <rdfs:label xml:lang="it">è risultato della formazione di</rdfs:label>
        <owl:versionInfo xml:lang="it">instabile</owl:versionInfo>
        <owl:versionInfo xml:lang="en">unstable</owl:versionInfo>
    </owl:ObjectProperty>
    


    <!-- https://w3id.org/ecodigit/ontology/eas/issuedBy -->

    <owl:ObjectProperty rdf:about="https://w3id.org/ecodigit/ontology/eas/issuedBy">
        <owl:inverseOf rdf:resource="https://w3id.org/ecodigit/ontology/eas/issues"/>
        <rdfs:domain rdf:resource="https://w3id.org/ecodigit/ontology/eas/Certification"/>
        <rdfs:range rdf:resource="https://w3id.org/italia/onto/COV/Organization"/>
        <rdfs:comment xml:lang="it">Questa proprietà associa una Certificazione con l&apos;Organizzazione che la rilascia.</rdfs:comment>
        <rdfs:comment xml:lang="en">This property associates a Certification with the issuing Organization.</rdfs:comment>
        <rdfs:label xml:lang="en">certification issued by</rdfs:label>
        <rdfs:label xml:lang="it">certificazione rilasciata da</rdfs:label>
        <owl:versionInfo xml:lang="it">instabile</owl:versionInfo>
        <owl:versionInfo xml:lang="en">unstable</owl:versionInfo>
    </owl:ObjectProperty>
    


    <!-- https://w3id.org/ecodigit/ontology/eas/issues -->

    <owl:ObjectProperty rdf:about="https://w3id.org/ecodigit/ontology/eas/issues">
        <rdfs:domain rdf:resource="https://w3id.org/italia/onto/COV/Organization"/>
        <rdfs:range rdf:resource="https://w3id.org/ecodigit/ontology/eas/Certification"/>
        <rdfs:comment xml:lang="it">Questa proprietà associa un&apos;Organizzazione con la Certificazione che essa rilascia.</rdfs:comment>
        <rdfs:comment xml:lang="en">This property associates an Organization with the Certification that it issues.</rdfs:comment>
        <rdfs:label xml:lang="en">issues certification</rdfs:label>
        <rdfs:label xml:lang="it">rilascia certificazione</rdfs:label>
        <owl:versionInfo xml:lang="it">instabile</owl:versionInfo>
        <owl:versionInfo xml:lang="en">unstable</owl:versionInfo>
    </owl:ObjectProperty>
    


    <!-- https://w3id.org/ecodigit/ontology/eas/leadsTo -->

    <owl:ObjectProperty rdf:about="https://w3id.org/ecodigit/ontology/eas/leadsTo">
        <rdfs:domain rdf:resource="https://w3id.org/ecodigit/ontology/eas/Examination"/>
        <rdfs:range rdf:resource="https://w3id.org/ecodigit/ontology/eas/Certification"/>
        <rdfs:comment xml:lang="it">Questa proprietà permette di associare la situazione del superamento di un Esame con la Certificazione ottenuta.</rdfs:comment>
        <rdfs:comment xml:lang="en">This property allows you to associate the situation of passing an Exam with the Certification obtained.</rdfs:comment>
        <rdfs:label xml:lang="en">leads to the achievement of</rdfs:label>
        <rdfs:label xml:lang="it">porta al conseguimento di</rdfs:label>
        <owl:versionInfo xml:lang="it">instabile</owl:versionInfo>
        <owl:versionInfo xml:lang="en">unstable</owl:versionInfo>
    </owl:ObjectProperty>
    


    <!-- https://w3id.org/ecodigit/ontology/eas/providedBy -->

    <owl:ObjectProperty rdf:about="https://w3id.org/ecodigit/ontology/eas/providedBy">
        <owl:inverseOf rdf:resource="https://w3id.org/ecodigit/ontology/eas/provides"/>
        <rdfs:domain rdf:resource="https://w3id.org/ecodigit/ontology/eas/Training"/>
        <rdfs:range rdf:resource="https://w3id.org/italia/onto/COV/Organization"/>
        <rdfs:comment xml:lang="it">Questa proprietà permette di associare una situazione di Formazione con l&apos;Organizzazione che la eroga.</rdfs:comment>
        <rdfs:comment xml:lang="en">This property associates a Training situation with the Organization providing it.</rdfs:comment>
        <rdfs:label xml:lang="it">offerta da</rdfs:label>
        <rdfs:label xml:lang="en">provided by</rdfs:label>
        <owl:versionInfo xml:lang="it">instabile</owl:versionInfo>
        <owl:versionInfo xml:lang="en">unstable</owl:versionInfo>
    </owl:ObjectProperty>
    


    <!-- https://w3id.org/ecodigit/ontology/eas/provides -->

    <owl:ObjectProperty rdf:about="https://w3id.org/ecodigit/ontology/eas/provides">
        <rdfs:domain rdf:resource="https://w3id.org/italia/onto/COV/Organization"/>
        <rdfs:range rdf:resource="https://w3id.org/ecodigit/ontology/eas/Training"/>
        <rdfs:comment xml:lang="it">Questa è la proprietà inversa di &apos;è offerta da&apos;.</rdfs:comment>
        <rdfs:comment xml:lang="en">This is the inverse object property of &apos;provided by&apos;.</rdfs:comment>
        <rdfs:label xml:lang="it">offre</rdfs:label>
        <rdfs:label xml:lang="en">provides</rdfs:label>
        <owl:versionInfo xml:lang="it">instabile</owl:versionInfo>
        <owl:versionInfo xml:lang="en">unstable</owl:versionInfo>
    </owl:ObjectProperty>
    


    <!-- 
    ///////////////////////////////////////////////////////////////////////////////////////
    //
    // Data properties
    //
    ///////////////////////////////////////////////////////////////////////////////////////
     -->

    


    <!-- https://w3id.org/ecodigit/ontology/eas/issueDate -->

    <owl:DatatypeProperty rdf:about="https://w3id.org/ecodigit/ontology/eas/issueDate">
        <rdfs:subPropertyOf rdf:resource="https://w3id.org/italia/onto/TI/date"/>
        <rdfs:domain rdf:resource="https://w3id.org/ecodigit/ontology/eas/Certification"/>
        <rdfs:range rdf:resource="http://www.w3.org/2001/XMLSchema#date"/>
    </owl:DatatypeProperty>
    


    <!-- 
    ///////////////////////////////////////////////////////////////////////////////////////
    //
    // Classes
    //
    ///////////////////////////////////////////////////////////////////////////////////////
     -->

    


    <!-- http://purl.org/ontology/bibo/Thesis -->

    <owl:Class rdf:about="http://purl.org/ontology/bibo/Thesis"/>
    


    <!-- http://xmlns.com/foaf/0.1/Agent -->

    <owl:Class rdf:about="http://xmlns.com/foaf/0.1/Agent"/>
    


    <!-- https://w3id.org/ecodigit/ontology/eas/CERFLevel -->

    <owl:Class rdf:about="https://w3id.org/ecodigit/ontology/eas/CERFLevel">
        <rdfs:subClassOf rdf:resource="https://w3id.org/ecodigit/ontology/eas/Level"/>
        <rdfs:comment xml:lang="it">Questa classe rappresenta i sei livelli (A1, A2, B1, B2, C1, C2) previsti dal Quadro comune europeo di riferimento per la conoscenza delle lingue (QCER), in inglese Common European Framework of Reference for Languages (CEFR).</rdfs:comment>
        <rdfs:label xml:lang="en">CERF Level</rdfs:label>
        <rdfs:label xml:lang="it">Livello CERF</rdfs:label>
        <owl:versionInfo xml:lang="it">instabile</owl:versionInfo>
        <owl:versionInfo xml:lang="en">unstable</owl:versionInfo>
    </owl:Class>
    


    <!-- https://w3id.org/ecodigit/ontology/eas/Certification -->

    <owl:Class rdf:about="https://w3id.org/ecodigit/ontology/eas/Certification">
        <rdfs:subClassOf rdf:resource="https://w3id.org/italia/onto/l0/Object"/>
        <rdfs:subClassOf>
            <owl:Restriction>
                <owl:onProperty rdf:resource="https://w3id.org/ecodigit/ontology/eas/attests"/>
                <owl:allValuesFrom>
                    <owl:Class>
                        <owl:unionOf rdf:parseType="Collection">
                            <rdf:Description rdf:about="https://w3id.org/ecodigit/ontology/eas/Level"/>
                            <rdf:Description rdf:about="https://w3id.org/ecodigit/ontology/eas/LevelInActivity"/>
                        </owl:unionOf>
                    </owl:Class>
                </owl:allValuesFrom>
            </owl:Restriction>
        </rdfs:subClassOf>
        <rdfs:subClassOf>
            <owl:Restriction>
                <owl:onProperty rdf:resource="https://w3id.org/ecodigit/ontology/eas/issueDate"/>
                <owl:allValuesFrom rdf:resource="http://www.w3.org/2001/XMLSchema#date"/>
            </owl:Restriction>
        </rdfs:subClassOf>
        <rdfs:comment xml:lang="it">Questa classe rappresenta la documentazione, che può essere istituzionale o autodichiarata, relativa alla Certificazione del Livello di Istruzione e Competenza di una persona.</rdfs:comment>
        <rdfs:comment xml:lang="en">This class represents the documentation, which can be institutional or self-declared, related to the Certification of the Level of Education and Expertise of a person.</rdfs:comment>
        <rdfs:label xml:lang="en">Certification</rdfs:label>
        <rdfs:label>Certificazione</rdfs:label>
        <owl:versionInfo xml:lang="it">instabile</owl:versionInfo>
        <owl:versionInfo xml:lang="en">unstable</owl:versionInfo>
    </owl:Class>
    


    <!-- https://w3id.org/ecodigit/ontology/eas/Examination -->

    <owl:Class rdf:about="https://w3id.org/ecodigit/ontology/eas/Examination">
        <rdfs:subClassOf rdf:resource="https://w3id.org/italia/onto/TI/TimeIndexedEvent"/>
        <rdfs:subClassOf>
            <owl:Restriction>
                <owl:onProperty rdf:resource="https://w3id.org/ecodigit/ontology/eas/leadsTo"/>
                <owl:someValuesFrom rdf:resource="https://w3id.org/ecodigit/ontology/eas/Certification"/>
            </owl:Restriction>
        </rdfs:subClassOf>
        <rdfs:subClassOf>
            <owl:Restriction>
                <owl:onProperty rdf:resource="https://w3id.org/ecodigit/ontology/grade/hasGrade"/>
                <owl:someValuesFrom rdf:resource="https://w3id.org/ecodigit/ontology/grade/Grade"/>
            </owl:Restriction>
        </rdfs:subClassOf>
        <rdfs:subClassOf>
            <owl:Restriction>
                <owl:onProperty rdf:resource="https://w3id.org/ecodigit/ontology/eas/hasTrainingOutcome"/>
                <owl:allValuesFrom rdf:resource="http://purl.org/ontology/bibo/Thesis"/>
            </owl:Restriction>
        </rdfs:subClassOf>
        <rdfs:comment xml:lang="it">Questa classe rappresenta la situazione di Esame, che accerta la preparazione della Persona che ha seguito l&apos;Esperienza formativa, e porta al conseguimento di una Certificazione.</rdfs:comment>
        <rdfs:comment xml:lang="en">This class represents the situation of an Examination, which aims to verify the preparation of the Person who followed the Training experience, leading to the achievement of a Certification.</rdfs:comment>
        <rdfs:label xml:lang="it">Esame</rdfs:label>
        <rdfs:label xml:lang="en">Examination</rdfs:label>
        <owl:versionInfo xml:lang="it">instabile</owl:versionInfo>
        <owl:versionInfo xml:lang="en">unstable</owl:versionInfo>
    </owl:Class>
    


    <!-- https://w3id.org/ecodigit/ontology/eas/ExpertiseAndSkill -->

    <owl:Class rdf:about="https://w3id.org/ecodigit/ontology/eas/ExpertiseAndSkill">
        <rdfs:subClassOf rdf:resource="https://w3id.org/italia/onto/l0/Characteristic"/>
        <rdfs:subClassOf>
            <owl:Restriction>
                <owl:onProperty rdf:resource="https://w3id.org/ecodigit/ontology/eas/hasCertification"/>
                <owl:someValuesFrom>
                    <owl:Class>
                        <owl:unionOf rdf:parseType="Collection">
                            <rdf:Description rdf:about="https://w3id.org/ecodigit/ontology/eas/IstitutionalCertification"/>
                            <rdf:Description rdf:about="https://w3id.org/ecodigit/ontology/eas/SelfCertification"/>
                        </owl:unionOf>
                    </owl:Class>
                </owl:someValuesFrom>
            </owl:Restriction>
        </rdfs:subClassOf>
        <rdfs:comment xml:lang="it">Questa classe rappresenta l&apos;esperienza e competenza che una persona ha acquisito grazie a una Esperienza formativa, che può essere certificata o meno.</rdfs:comment>
        <rdfs:comment xml:lang="en">This class represents the Expertise and competence gained by a Person thanks to a Training, which may be certified or not.</rdfs:comment>
        <rdfs:label xml:lang="it">Esperienza e Competenza</rdfs:label>
        <rdfs:label xml:lang="en">Expertise and Skill</rdfs:label>
        <owl:versionInfo xml:lang="it">instabile</owl:versionInfo>
        <owl:versionInfo xml:lang="en">unstable</owl:versionInfo>
        <prov:wasInfluencedBy rdf:resource="https://www.eurocris.org/ontologies/cerif/#ExpSkill"/>
    </owl:Class>
    


    <!-- https://w3id.org/ecodigit/ontology/eas/FinalExamination -->

    <owl:Class rdf:about="https://w3id.org/ecodigit/ontology/eas/FinalExamination">
        <rdfs:subClassOf rdf:resource="https://w3id.org/ecodigit/ontology/eas/Examination"/>
        <rdfs:comment xml:lang="it">Questa classe rappresenta un Esame previsto al termine di un&apos;Esperienza formativa che permette di ottenere una Certificazione. Tale Esame può avere come risultato la preparazione di una Tesi.</rdfs:comment>
        <rdfs:comment xml:lang="en">This class represents an Examination scheduled at the end of a Training experience that leads to a Certification. This Examination may result in the preparation of a Thesis.</rdfs:comment>
        <rdfs:label xml:lang="it">Esame Finale</rdfs:label>
        <rdfs:label xml:lang="en">Final Examination</rdfs:label>
        <owl:versionInfo xml:lang="it">instabile</owl:versionInfo>
        <owl:versionInfo xml:lang="en">unstable</owl:versionInfo>
    </owl:Class>
    


    <!-- https://w3id.org/ecodigit/ontology/eas/IstitutionalCertification -->

    <owl:Class rdf:about="https://w3id.org/ecodigit/ontology/eas/IstitutionalCertification">
        <rdfs:subClassOf rdf:resource="https://w3id.org/ecodigit/ontology/eas/Certification"/>
        <rdfs:subClassOf>
            <owl:Restriction>
                <owl:onProperty rdf:resource="https://w3id.org/ecodigit/ontology/eas/issuedBy"/>
                <owl:someValuesFrom rdf:resource="https://w3id.org/italia/onto/COV/Organization"/>
            </owl:Restriction>
        </rdfs:subClassOf>
        <owl:disjointWith rdf:resource="https://w3id.org/ecodigit/ontology/eas/SelfCertification"/>
        <rdfs:comment xml:lang="it">Questa classe rappresenta le Certificazioni emesse ufficialmente da una Organizzazione.</rdfs:comment>
        <rdfs:comment xml:lang="en">This class represents the Certifications officially issued by an Organization.</rdfs:comment>
        <rdfs:label xml:lang="it">Certificazione istituzionale</rdfs:label>
        <rdfs:label xml:lang="en">Istitutional Certification</rdfs:label>
        <owl:versionInfo xml:lang="it">instabile</owl:versionInfo>
        <owl:versionInfo xml:lang="en">unstable</owl:versionInfo>
    </owl:Class>
    


    <!-- https://w3id.org/ecodigit/ontology/eas/LanguageActivity -->

    <owl:Class rdf:about="https://w3id.org/ecodigit/ontology/eas/LanguageActivity">
        <rdfs:subClassOf rdf:resource="https://w3id.org/italia/onto/l0/Activity"/>
        <rdfs:label xml:lang="it">Attività linguistiche</rdfs:label>
    </owl:Class>
    


    <!-- https://w3id.org/ecodigit/ontology/eas/LanguageSkill -->

    <owl:Class rdf:about="https://w3id.org/ecodigit/ontology/eas/LanguageSkill">
        <rdfs:subClassOf rdf:resource="https://w3id.org/ecodigit/ontology/eas/ExpertiseAndSkill"/>
        <rdfs:subClassOf>
            <owl:Restriction>
                <owl:onProperty rdf:resource="https://w3id.org/italia/onto/Language/hasLanguage"/>
                <owl:someValuesFrom rdf:resource="https://w3id.org/italia/onto/Language/Language"/>
            </owl:Restriction>
        </rdfs:subClassOf>
    </owl:Class>
    


    <!-- https://w3id.org/ecodigit/ontology/eas/Level -->

    <owl:Class rdf:about="https://w3id.org/ecodigit/ontology/eas/Level">
        <rdfs:subClassOf rdf:resource="https://w3id.org/italia/onto/l0/Characteristic"/>
        <rdfs:comment xml:lang="it">Questa classe rappresenta il Livello di istruzione e competenza attestato da una Certificazione.</rdfs:comment>
        <rdfs:comment xml:lang="en">This class represents the Level of Education and Expertise attested by a Certification.</rdfs:comment>
        <rdfs:label xml:lang="en">Level</rdfs:label>
        <rdfs:label xml:lang="it">Livello</rdfs:label>
        <owl:versionInfo xml:lang="it">instabile</owl:versionInfo>
        <owl:versionInfo xml:lang="en">unstable</owl:versionInfo>
        <prov:wasInfluencedBy rdf:resource="http://www.bbc.co.uk/ontologies/curriculum/Level"/>
    </owl:Class>
    


    <!-- https://w3id.org/ecodigit/ontology/eas/LevelInActivity -->

    <owl:Class rdf:about="https://w3id.org/ecodigit/ontology/eas/LevelInActivity">
        <rdfs:subClassOf rdf:resource="https://w3id.org/italia/onto/l0/Characteristic"/>
        <rdfs:subClassOf>
            <owl:Restriction>
                <owl:onProperty rdf:resource="https://w3id.org/ecodigit/ontology/eas/hasActivity"/>
                <owl:someValuesFrom rdf:resource="https://w3id.org/italia/onto/l0/Activity"/>
            </owl:Restriction>
        </rdfs:subClassOf>
        <rdfs:subClassOf>
            <owl:Restriction>
                <owl:onProperty rdf:resource="https://w3id.org/ecodigit/ontology/eas/hasLevel"/>
                <owl:someValuesFrom rdf:resource="https://w3id.org/ecodigit/ontology/eas/Level"/>
            </owl:Restriction>
        </rdfs:subClassOf>
        <rdfs:comment xml:lang="it">Questa classe rappresenta il Livello attestato da un Certificato in una certa Attività. Questa classe è una reificazione della proprietà eas:attests. La classe permette di specificare oltre al livello attestato una eventuale attività a cui si riferisce il livello. La modellazione di questa classe è influenzata dal Common European Framework of Reference for Languages (CERF). In CERF è possibile esprimere il fatto che una persona ha raggiunto un certo livello (e.g. B1) in una attività del linguaggio (e.g. Listening Comprehension) e un altro livello (e.g. C1) in un&apos;altra attività del linguaggio (e.g. Reading Compehension).</rdfs:comment>
        <rdfs:label xml:lang="en">Level in Activity</rdfs:label>
        <rdfs:label xml:lang="it">Livello in Attività</rdfs:label>
        <owl:versionInfo xml:lang="it">unstable</owl:versionInfo>
    </owl:Class>
    


    <!-- https://w3id.org/ecodigit/ontology/eas/SelfCertification -->

    <owl:Class rdf:about="https://w3id.org/ecodigit/ontology/eas/SelfCertification">
        <rdfs:subClassOf rdf:resource="https://w3id.org/ecodigit/ontology/eas/Certification"/>
        <rdfs:comment xml:lang="it">Questa classe rappresenta le Autocertificazioni redatte da una Persona sotto la propria responsabilità a norma di legge.</rdfs:comment>
        <rdfs:comment xml:lang="en">This class represents the Self-certifications drawn up by a Person under his own responsibility according to the law.</rdfs:comment>
        <rdfs:label xml:lang="it">Autocertificazione</rdfs:label>
        <rdfs:label xml:lang="en">Self-certification</rdfs:label>
        <owl:versionInfo xml:lang="it">instabile</owl:versionInfo>
        <owl:versionInfo xml:lang="en">unstable</owl:versionInfo>
    </owl:Class>
    


    <!-- https://w3id.org/ecodigit/ontology/eas/Training -->

    <owl:Class rdf:about="https://w3id.org/ecodigit/ontology/eas/Training">
        <rdfs:subClassOf rdf:resource="https://w3id.org/italia/onto/TI/TimeIndexedEvent"/>
        <rdfs:subClassOf>
            <owl:Restriction>
                <owl:onProperty rdf:resource="https://w3id.org/ecodigit/ontology/eas/isAttendedBy"/>
                <owl:someValuesFrom rdf:resource="http://xmlns.com/foaf/0.1/Person"/>
            </owl:Restriction>
        </rdfs:subClassOf>
        <rdfs:subClassOf>
            <owl:Restriction>
                <owl:onProperty rdf:resource="https://w3id.org/ecodigit/ontology/eas/providedBy"/>
                <owl:someValuesFrom rdf:resource="http://xmlns.com/foaf/0.1/Organization"/>
            </owl:Restriction>
        </rdfs:subClassOf>
        <rdfs:subClassOf>
            <owl:Restriction>
                <owl:onProperty rdf:resource="https://w3id.org/ecodigit/ontology/eas/hasCertification"/>
                <owl:allValuesFrom rdf:resource="https://w3id.org/ecodigit/ontology/eas/Certification"/>
            </owl:Restriction>
        </rdfs:subClassOf>
        <rdfs:subClassOf>
            <owl:Restriction>
                <owl:onProperty rdf:resource="https://w3id.org/ecodigit/ontology/eas/includesAnExamination"/>
                <owl:allValuesFrom rdf:resource="https://w3id.org/ecodigit/ontology/eas/Examination"/>
            </owl:Restriction>
        </rdfs:subClassOf>
        <rdfs:comment xml:lang="it">La classe rappresenta le Esperienze formative, erogate da una Organizzazione, a cui una Persona ha partecipato. Esse possono prevedere o meno un Esame con relativa Certificazione.</rdfs:comment>
        <rdfs:comment xml:lang="en">The class represents the Training experiences, provided by an Organization and attended by a Person. They may include or not an Examination with a Certification.</rdfs:comment>
        <rdfs:label xml:lang="it">Esperienza Formativa</rdfs:label>
        <rdfs:label xml:lang="en">Training</rdfs:label>
        <owl:versionInfo xml:lang="it">instabile</owl:versionInfo>
        <owl:versionInfo xml:lang="en">unstable</owl:versionInfo>
    </owl:Class>
    


    <!-- https://w3id.org/italia/onto/COV/Organization -->

    <owl:Class rdf:about="https://w3id.org/italia/onto/COV/Organization"/>
    


    <!-- 
    ///////////////////////////////////////////////////////////////////////////////////////
    //
    // Individuals
    //
    ///////////////////////////////////////////////////////////////////////////////////////
     -->

    


    <!-- https://w3id.org/ecodigit/ontology/eas/A1 -->

    <owl:NamedIndividual rdf:about="https://w3id.org/ecodigit/ontology/eas/A1">
        <rdf:type rdf:resource="https://w3id.org/ecodigit/ontology/eas/CERFLevel"/>
        <rdfs:comment xml:lang="it">Questo individuo rappresenta il livello base A1 del Common European Framework of Reference for Languages (CEFR).</rdfs:comment>
        <rdfs:comment xml:lang="en">This individual represents the A1 beginner level of the Common European Framework of Reference for Languages ​​(CEFR).</rdfs:comment>
        <rdfs:label xml:lang="en">Level A1</rdfs:label>
        <rdfs:label xml:lang="it">Livello A1</rdfs:label>
        <owl:versionInfo xml:lang="it">instabile</owl:versionInfo>
        <owl:versionInfo xml:lang="en">unstable</owl:versionInfo>
    </owl:NamedIndividual>
    


    <!-- https://w3id.org/ecodigit/ontology/eas/A2 -->

    <owl:NamedIndividual rdf:about="https://w3id.org/ecodigit/ontology/eas/A2">
        <rdf:type rdf:resource="https://w3id.org/ecodigit/ontology/eas/CERFLevel"/>
        <rdfs:comment xml:lang="it">Questo individuo rappresenta il livello elementare A2 del Common European Framework of Reference for Languages (CEFR).</rdfs:comment>
        <rdfs:comment xml:lang="en">This individual represents the A2 elementary level of the Common European Framework of Reference for Languages ​​(CEFR).</rdfs:comment>
        <rdfs:label xml:lang="en">Level A2</rdfs:label>
        <rdfs:label xml:lang="it">Livello A2</rdfs:label>
        <owl:versionInfo xml:lang="it">instabile</owl:versionInfo>
        <owl:versionInfo xml:lang="en">unstable</owl:versionInfo>
    </owl:NamedIndividual>
    


    <!-- https://w3id.org/ecodigit/ontology/eas/B1 -->

    <owl:NamedIndividual rdf:about="https://w3id.org/ecodigit/ontology/eas/B1">
        <rdf:type rdf:resource="https://w3id.org/ecodigit/ontology/eas/CERFLevel"/>
        <rdfs:comment xml:lang="it">Questo individuo rappresenta il livello intermedio B1 del Common European Framework of Reference for Languages (CEFR).</rdfs:comment>
        <rdfs:comment xml:lang="en">This individual represents the B1 intermediate level of the Common European Framework of Reference for Languages ​​(CEFR).</rdfs:comment>
        <rdfs:label xml:lang="en">Level B1</rdfs:label>
        <rdfs:label xml:lang="it">Livello B1</rdfs:label>
        <owl:versionInfo xml:lang="it">instabile</owl:versionInfo>
        <owl:versionInfo xml:lang="en">unstable</owl:versionInfo>
    </owl:NamedIndividual>
    


    <!-- https://w3id.org/ecodigit/ontology/eas/B2 -->

    <owl:NamedIndividual rdf:about="https://w3id.org/ecodigit/ontology/eas/B2">
        <rdf:type rdf:resource="https://w3id.org/ecodigit/ontology/eas/CERFLevel"/>
        <rdfs:comment xml:lang="it">Questo individuo rappresenta il livello intermedio superiore B2 del Common European Framework of Reference for Languages (CEFR).</rdfs:comment>
        <rdfs:comment xml:lang="en">This individual represents the B2 upper intermediate level of the Common European Framework of Reference for Languages ​​(CEFR).</rdfs:comment>
        <rdfs:label xml:lang="en">Level B2</rdfs:label>
        <rdfs:label xml:lang="it">Livello B2</rdfs:label>
        <owl:versionInfo xml:lang="it">instabile</owl:versionInfo>
        <owl:versionInfo xml:lang="en">unstable</owl:versionInfo>
    </owl:NamedIndividual>
    


    <!-- https://w3id.org/ecodigit/ontology/eas/C1 -->

    <owl:NamedIndividual rdf:about="https://w3id.org/ecodigit/ontology/eas/C1">
        <rdf:type rdf:resource="https://w3id.org/ecodigit/ontology/eas/CERFLevel"/>
        <rdfs:comment xml:lang="it">Questo individuo rappresenta il livello avanzato C1 del Common European Framework of Reference for Languages (CEFR).</rdfs:comment>
        <rdfs:comment xml:lang="en">This individual represents the C1 advanced level of the Common European Framework of Reference for Languages ​​(CEFR).</rdfs:comment>
        <rdfs:label xml:lang="en">Level C1</rdfs:label>
        <rdfs:label xml:lang="it">Livello C1</rdfs:label>
        <owl:versionInfo xml:lang="it">instabile</owl:versionInfo>
        <owl:versionInfo xml:lang="en">unstable</owl:versionInfo>
    </owl:NamedIndividual>
    


    <!-- https://w3id.org/ecodigit/ontology/eas/C2 -->

    <owl:NamedIndividual rdf:about="https://w3id.org/ecodigit/ontology/eas/C2">
        <rdf:type rdf:resource="https://w3id.org/ecodigit/ontology/eas/CERFLevel"/>
        <rdfs:comment xml:lang="it">Questo individuo rappresenta il livello di padronanza C2 del Common European Framework of Reference for Languages (CEFR).</rdfs:comment>
        <rdfs:comment xml:lang="en">This individual represents the C2 proficiency level of the Common European Framework of Reference for Languages ​​(CEFR).</rdfs:comment>
        <rdfs:label xml:lang="en">Level C2</rdfs:label>
        <rdfs:label xml:lang="it">Livello C2</rdfs:label>
        <owl:versionInfo xml:lang="it">instabile</owl:versionInfo>
        <owl:versionInfo xml:lang="en">unstable</owl:versionInfo>
    </owl:NamedIndividual>
    


    <!-- https://w3id.org/ecodigit/ontology/eas/Interaction -->

    <owl:NamedIndividual rdf:about="https://w3id.org/ecodigit/ontology/eas/Interaction">
        <rdf:type rdf:resource="https://w3id.org/ecodigit/ontology/eas/LanguageActivity"/>
    </owl:NamedIndividual>
    


    <!-- https://w3id.org/ecodigit/ontology/eas/ListeningComprehension -->

    <owl:NamedIndividual rdf:about="https://w3id.org/ecodigit/ontology/eas/ListeningComprehension">
        <rdf:type rdf:resource="https://w3id.org/ecodigit/ontology/eas/LanguageActivity"/>
    </owl:NamedIndividual>
    


    <!-- https://w3id.org/ecodigit/ontology/eas/Production -->

    <owl:NamedIndividual rdf:about="https://w3id.org/ecodigit/ontology/eas/Production">
        <rdf:type rdf:resource="https://w3id.org/ecodigit/ontology/eas/LanguageActivity"/>
    </owl:NamedIndividual>
    


    <!-- https://w3id.org/ecodigit/ontology/eas/ReadingComprehension -->

    <owl:NamedIndividual rdf:about="https://w3id.org/ecodigit/ontology/eas/ReadingComprehension">
        <rdf:type rdf:resource="https://w3id.org/ecodigit/ontology/eas/LanguageActivity"/>
    </owl:NamedIndividual>
    


    <!-- https://w3id.org/ecodigit/ontology/eas/Reception -->

    <owl:NamedIndividual rdf:about="https://w3id.org/ecodigit/ontology/eas/Reception">
        <rdf:type rdf:resource="https://w3id.org/ecodigit/ontology/eas/LanguageActivity"/>
    </owl:NamedIndividual>
    


    <!-- https://w3id.org/ecodigit/ontology/eas/SpokenInteraction -->

    <owl:NamedIndividual rdf:about="https://w3id.org/ecodigit/ontology/eas/SpokenInteraction">
        <rdf:type rdf:resource="https://w3id.org/ecodigit/ontology/eas/LanguageActivity"/>
    </owl:NamedIndividual>
    


    <!-- https://w3id.org/ecodigit/ontology/eas/SpokenProduction -->

    <owl:NamedIndividual rdf:about="https://w3id.org/ecodigit/ontology/eas/SpokenProduction">
        <rdf:type rdf:resource="https://w3id.org/ecodigit/ontology/eas/LanguageActivity"/>
    </owl:NamedIndividual>
    


    <!-- https://w3id.org/ecodigit/ontology/eas/WrittenInteraction -->

    <owl:NamedIndividual rdf:about="https://w3id.org/ecodigit/ontology/eas/WrittenInteraction">
        <rdf:type rdf:resource="https://w3id.org/ecodigit/ontology/eas/LanguageActivity"/>
    </owl:NamedIndividual>
    


    <!-- https://w3id.org/ecodigit/ontology/eas/WrittenProduction -->

    <owl:NamedIndividual rdf:about="https://w3id.org/ecodigit/ontology/eas/WrittenProduction">
        <rdf:type rdf:resource="https://w3id.org/ecodigit/ontology/eas/LanguageActivity"/>
    </owl:NamedIndividual>
</rdf:RDF>



<!-- Generated by the OWL API (version 4.5.9.2019-02-01T07:24:44Z) https://github.com/owlcs/owlapi -->

